GroundMapsHelpers.v
@@ -1,0 +1,593 @@
+From Coq Require Import String List Arith.
+
+From VeriFGH Require Import DatalogProps MoreOrders DatalogSemantics.
+Import RelSemantics.
+
+Ltac negate_negated H :=
+                let Ht := type of H in
+                match Ht with
+                | ~ ?y =>
+                    let Y := fresh "Y" in
+                    assert (Y: y)
+                end.
+
+
+Lemma ground_maps_MapsTo_implies_In :
+  forall (g: gm_type) (x: string) (e: list (list ground_types)),
+    ground_maps.MapsTo x e g ->
+    ground_maps.In x g.
+Proof.
+  intros. destruct g. unfold ground_maps.MapsTo in H. unfold ground_maps.In. unfold ground_maps.Raw.PX.In. unfold ground_maps.Raw.PX.MapsTo in *. exists e. eassumption.
+Qed.
+
+Lemma ground_maps_add_iff :
+  forall (g: gm_type) (x x0: string) (l: list (list ground_types)),
+    ground_maps.In x (ground_maps.add x0 l g) <->
+      x = x0 \/ ground_maps.In x g.
+Proof.
+  destruct g. rename this into g.
+  induction g; split; intros.
+  - invs H.
+    invs H0.
+    + invs H2. simpl in *. subst.
+      invs H1. left. reflexivity.
+    + invs H2.
+  - destruct H.
+    + subst. unfold ground_maps.add. simpl. unfold ground_maps.In. simpl. unfold ground_maps.Raw.PX.In.
+      exists l. econstructor. reflexivity.
+    + unfold ground_maps.In in H. unfold ground_maps.Raw.PX.In in H. destruct H.
+      invs H.
+  - invs NoDup.
+    specialize (IHg H3).
+    unfold ground_maps.add in IHg. simpl in IHg. unfold ground_maps.In in IHg. simpl in IHg.
+    
+    unfold ground_maps.add in H. simpl in H.
+    destruct a.
+    pose proof (String_as_OT.eq_dec).
+    specialize (H0 x0 s).
+    destruct H0.
+    + subst.
+      unfold ground_maps.In in H. simpl in H. destruct (String_as_OT.eq_dec s s).
+      * destruct (String_as_OT.eq_dec x s).
+        -- left. eauto.
+        -- right. unfold ground_maps.In. simpl.
+           unfold ground_maps.Raw.PX.In in H. destruct H.
+           invs H.
+           ++ invs H1. simpl in *. subst. invs H0.
+              unfold ground_maps.Raw.PX.In. exists g0. econstructor. reflexivity.
+           ++ unfold ground_maps.Raw.PX.In.
+              exists x0.
+              unfold ground_maps.Raw.PX.MapsTo.
+              right. eassumption.
+      * congruence.
+    + unfold ground_maps.In in H. simpl in H. destruct (String_as_OT.eq_dec x0 s); try congruence.
+      unfold ground_maps.Raw.PX.In in H.
+      destruct H.
+      destruct (string_dec x x0); subst.
+      * left. eauto.
+      * right. unfold ground_maps.In. simpl. unfold ground_maps.Raw.PX.In.
+        invs H.
+        -- exists x1. invs H1. simpl in *. invs H0.
+           econstructor. reflexivity.
+        -- unfold ground_maps.Raw.PX.In in IHg. unfold ground_maps.Raw.PX.MapsTo in IHg. unfold ground_maps.Raw.PX.MapsTo.
+           specialize (IHg x x0 l).
+           destruct IHg.
+           assert (exists e,  SetoidList.InA
+                           (ground_maps.Raw.PX.eqke (elt:=list (list ground_types))) (
+                             x, e) (ground_maps.Raw.add x0 l g)).
+           exists x1. eassumption.
+           eapply H0 in H5. destruct H5.
+           congruence.
+           destruct H5. exists x2. right. eassumption.
+  - destruct H.
+    + subst. unfold ground_maps.add. simpl. destruct a.
+      unfold ground_maps.In. simpl. destruct (String_as_OT.eq_dec x0 s).
+      * subst. unfold ground_maps.Raw.PX.In. exists l. econstructor. reflexivity.
+      * unfold ground_maps.Raw.PX.In.
+        unfold ground_maps.In in IHg. simpl in IHg. unfold ground_maps.Raw.PX.In in IHg.
+        unfold ground_maps.Raw.PX.MapsTo in IHg.
+        assert (exists e,
+                   SetoidList.InA
+                     (ground_maps.Raw.PX.eqke (elt:=list (list ground_types)))
+                     (x0, e) (ground_maps.Raw.add x0 l g)).
+        eapply IHg.  invs NoDup. eauto.
+        left. reflexivity.
+        destruct H.
+        invs H.
+        -- destruct y.
+           invs H1. simpl in *. invs H2.
+           rewrite H0.
+           exists l1. right. eassumption.
+        -- rewrite H0. destruct y.
+           exists x.
+           right. rewrite <- H0. right. eauto.
+    + unfold ground_maps.In in *.
+      simpl in *. destruct a.
+      destruct (String_as_OT.eq_dec x0 s).
+      * subst. destruct (String_as_OT.eq_dec x s).
+        -- subst. unfold ground_maps.Raw.PX.In in *. unfold ground_maps.Raw.PX.MapsTo in *. exists l. left. reflexivity.
+        -- unfold ground_maps.Raw.PX.In in *.
+           unfold ground_maps.Raw.PX.MapsTo in *.
+           destruct H. invs H. invs H1. simpl in *. invs H0. congruence.
+           exists x0. right. eassumption.
+      * unfold ground_maps.Raw.PX.In in *.
+        unfold ground_maps.Raw.PX.MapsTo in *.
+        destruct H.
+        (* exists x1. *)
+        invs H.
+        -- invs H1. simpl in *. invs H0. exists g0. left. reflexivity.
+        -- assert (exists e,
+                      SetoidList.InA (ground_maps.Raw.PX.eqke (elt:=gt_set_type)) (
+                                       x, e) g).
+           exists x1. eassumption.
+           assert (x = x0 \/ exists (e: list (list ground_types)), SetoidList.InA (ground_maps.Raw.PX.eqke (elt:=gt_set_type)) (
+                                                                              x, e) g).
+           right. eassumption. invs NoDup.
+           specialize (IHg H6).
+           eapply IHg in H2.
+           pose proof (string_dec x s).
+           destruct H3.
+           ++ subst. exists g0. left. reflexivity.
+           ++ destruct H2. exists x2. right. eassumption.
+Qed.        
+
+
+Lemma ground_maps_raw_MapsTo_implies_In :
+  forall g x (l3: list (list ground_types)),
+  ground_maps.Raw.PX.MapsTo x l3
+                            (g) ->
+  ground_maps.Raw.PX.In x (g).
+Proof.
+  intros. unfold ground_maps.Raw.PX.In. exists l3. eassumption.
+Qed.
+
+Lemma ground_maps_eqke_inversion :
+  forall x0 (x l3: list (list ground_types)) s,
+    ground_maps.Raw.PX.eqke (x0, x) (s, l3) ->
+    x0 = s /\ x = l3.
+Proof.
+  intros. invs H. simpl in *. invc H0. split; reflexivity.
+Qed.
+
+Lemma ground_maps_raw_MapsTo_cons_iff :
+  forall g x0 s (l1 l2: list (list ground_types)),
+    ground_maps.Raw.PX.MapsTo x0 l1 ((s, l2) :: g) <->
+      (x0 = s /\ l1 = l2) \/ ground_maps.Raw.PX.MapsTo x0 l1 g.
+Proof.
+  induction g; split; intros.
+  - invs H. eapply ground_maps_eqke_inversion in H1. destruct H1; subst.
+    left. eauto.
+    invs H1.
+  - destruct H; try congruence.
+    destruct H; subst. econstructor. reflexivity.
+    invs H.
+  - invs H.
+    + eapply ground_maps_eqke_inversion in H1. destruct H1; subst.
+      left. eauto.
+    + unfold ground_maps.Raw.PX.MapsTo in IHg. destruct a.
+      eapply IHg in H1. destruct H1.
+      * destruct H0; subst.
+        invs H.
+        -- eapply ground_maps_eqke_inversion in H1. destruct H1; subst.
+           left; eauto.
+        -- invs H1.
+           ++ right. econstructor. reflexivity.
+           ++ right. unfold ground_maps.Raw.PX.MapsTo.
+              right. eassumption.
+      * right. unfold ground_maps.Raw.PX.MapsTo. right. eassumption.
+  - destruct H.
+    + destruct H; subst. econstructor. reflexivity.
+    + right. destruct a. eapply IHg in H. destruct H; [ destruct H; subst | ].
+      * left. reflexivity.
+      * right. eapply H.
+Qed.
+
+Lemma ground_maps_raw_In_cons_iff :
+  forall g x0 s (l3: list (list ground_types)),
+    ground_maps.Raw.PX.In x0 ((s, l3) :: g) <->
+      x0 = s \/ ground_maps.Raw.PX.In x0 g.
+Proof.
+  split; intros.
+  - unfold ground_maps.Raw.PX.In in H. destruct H.
+    eapply ground_maps_raw_MapsTo_cons_iff in H. destruct H.
+    + left. eapply H.
+    + right. unfold ground_maps.Raw.PX.MapsTo in H. unfold ground_maps.Raw.PX.In. exists x. eapply H.
+  - destruct H; subst.
+    + unfold ground_maps.Raw.PX.In. exists l3. left. reflexivity.
+    + unfold ground_maps.Raw.PX.In in *.
+      destruct H. unfold ground_maps.Raw.PX.MapsTo in *.
+      exists x. right. eauto.
+Qed.
+
+Print ground_maps.MapsTo.
+#[local]
+ Arguments ground_maps.MapsTo [elt]%type_scope x e m/.
+#[local]
+ Arguments ground_maps.add [elt]%type_scope x e m /.
+
+
+
+
+Lemma notIn_setoid_cons_subsets :
+  forall g x y,
+    ~
+       SetoidList.InA
+         (ground_maps.Raw.PX.eqk (elt:=list (list ground_types))) x
+         (y :: g) ->
+    ~
+       SetoidList.InA
+         (ground_maps.Raw.PX.eqk (elt:=list (list ground_types))) x
+         (g).
+Proof.
+  destruct g; intros.
+  - unfold not. intros. invs H0.
+  - unfold not. intros.
+    negate_negated H.
+    right. eauto. contradiction.
+Qed.
+         
+Lemma NoDup_setoid_cons_subsets :
+  forall g x y,
+  SetoidList.NoDupA
+         (ground_maps.Raw.PX.eqk (elt:=list (list ground_types)))
+         (x :: y :: g) ->
+  SetoidList.NoDupA
+         (ground_maps.Raw.PX.eqk (elt:=list (list ground_types)))
+         (x :: g) /\
+    SetoidList.NoDupA
+         (ground_maps.Raw.PX.eqk (elt:=list (list ground_types)))
+         (y :: g).
+Proof.
+  induction g; intros.
+  - split.
+    + econstructor. unfold not; intros. invs H0.
+      econstructor.
+    + econstructor. unfold not; intros. invs H0. econstructor.
+  - invs H.
+    split; eauto.
+    eapply notIn_setoid_cons_subsets in H2. invs H3. econstructor; eauto.
+Qed.
+Lemma ground_maps_cons_in_contradiction :
+  forall g (v1 l: list (list ground_types)) s,
+  SetoidList.InA
+         (ground_maps.Raw.PX.eqke (elt:=list (list ground_types))) (
+           s, v1) g ->
+  SetoidList.NoDupA
+            (ground_maps.Raw.PX.eqk (elt:=list (list ground_types)))
+            ((s, l) :: g) ->
+  False.
+Proof.
+  induction g; intros.
+  - invs H.
+  - invs H.
+    + destruct a. eapply ground_maps_eqke_inversion in H2. destruct H2; subst.
+      invs H0. negate_negated H3.
+      left. reflexivity.
+      congruence.
+    + eapply NoDup_setoid_cons_subsets in H0.
+      destruct H0.
+      invs H0.
+      eapply IHg.  eapply H2. eauto.
+Qed.
+
+      
+
+Lemma ground_maps_MapsTo_add_iff :
+  forall g x1 x2 (v1 v2: list (list ground_types)),
+    ground_maps.MapsTo x1 v1 (ground_maps.add x2 v2 g) <->
+      (x1 = x2 /\ v1 = v2) \/ (x1 <> x2 /\ ground_maps.MapsTo x1 v1 g).
+Proof.
+  destruct g. rename this into g. induction g; split; intros.
+  - simpl in H. simpl. invs H. eapply ground_maps_eqke_inversion in H1. left. eauto.
+    invs H1.
+  - destruct H; try invs H.
+    simpl. left. reflexivity.
+    invs H1.
+  - simpl in H. destruct a.
+    simpl. destruct (String_as_OT.eq_dec x2 s).
+    + subst. invs H.
+      * eapply ground_maps_eqke_inversion in H1. destruct H1; subst.
+        left; eauto.
+      * destruct (string_dec x1 s).
+        -- subst. invs H. eapply ground_maps_eqke_inversion in H2. destruct H2; subst.
+           left; eauto.
+           (* this is a contradiction, since
+              SetoidList.InA
+         (ground_maps.Raw.PX.eqke (elt:=list (list ground_types))) (
+         s, v1) g
+implies that s is a key of g, but
+SetoidList.NoDupA
+            (ground_maps.Raw.PX.eqk (elt:=list (list ground_types)))
+            ((s, l) :: g)
+implies that s is not a key of g
+            *)
+           eapply ground_maps_cons_in_contradiction in H2.
+           invs H2. eauto.
+        -- right. split; eauto.
+    + invs H.
+      * eapply ground_maps_eqke_inversion in H1. destruct H1; subst. right. split; try congruence.
+        left; eauto.
+      * eapply IHg in H1. destruct H1.
+        -- destruct H0; subst. left; eauto.
+        -- destruct H0. right. split; eauto.
+  - simpl. simpl in H. destruct a. destruct (String_as_OT.eq_dec x2 s).
+    + subst. destruct H.
+      * destruct H; subst. left. reflexivity.
+      * destruct H. invs H0.
+        -- eapply ground_maps_eqke_inversion in H2. destruct H2; congruence.
+        -- right. eauto.
+    + destruct H.
+      * destruct H; subst. right. eapply IHg. left. eauto.
+      * destruct H. invs H0.
+        -- eapply ground_maps_eqke_inversion in H2. destruct H2. subst.
+           left. reflexivity.
+        -- right. eapply IHg. right. eauto.
+           Unshelve.
+           ++ invs NoDup. eassumption.
+           ++ invs NoDup. eassumption.
+           ++ invs NoDup. eassumption.
+Qed.
+
+Lemma ground_maps_MapsTo_det :
+  forall g x (v1 v2: list (list ground_types)),
+    ground_maps.MapsTo x v1 g ->
+    ground_maps.MapsTo x v2 g ->
+    v1 = v2.
+Proof.
+  destruct g. rename this into g. induction g; intros.
+  - invs H.
+  - destruct a. invs NoDup. unfold ground_maps.MapsTo in *. simpl in H, H0.
+    eapply ground_maps_raw_MapsTo_cons_iff in H, H0.
+    destruct H, H0.
+    + destruct H. destruct H0. subst. reflexivity.
+    +  destruct H. subst. pose proof (ground_maps_cons_in_contradiction).
+       specialize (H g v2 l s H0 NoDup).
+       contradiction.
+    + destruct H0. subst.
+      pose proof (ground_maps_cons_in_contradiction g v1 l s H NoDup).
+      contradiction.
+    + simpl in IHg. eapply IHg; eauto.
+Qed.
+
+Lemma ground_maps_raw_MapsTo_add_iff :
+  forall g x1 x2 (v1 v2: list (list ground_types)),
+    SetoidList.NoDupA
+            (ground_maps.Raw.PX.eqk (elt:=list (list ground_types)))
+            g ->
+    ground_maps.Raw.PX.MapsTo x1 v1
+                              (ground_maps.Raw.add x2 v2 g) <->
+      (x1 = x2 /\ v1 = v2) \/ (x1 <> x2 /\ ground_maps.Raw.PX.MapsTo x1 v1 g).
+Proof.
+  pose proof (ground_maps_MapsTo_add_iff).
+  unfold ground_maps.MapsTo in H. simpl in H.
+  intros.
+  specialize (H ({| ground_maps.this := g; ground_maps.NoDup := H0 |})).
+  simpl in H. eapply H.
+Qed.
+
+Lemma ground_maps_raw_cons_add_commute :
+  forall g x0 x1 x l1 s g0,
+    SetoidList.NoDupA (ground_maps.Raw.PX.eqk (elt:=list (list ground_types)))
+                      ((s, g0) :: g) ->
+    x <> s ->
+    ground_maps.Raw.PX.MapsTo x0 x1
+                              ((s, g0) :: ground_maps.Raw.add x l1 g) ->
+    ground_maps.Raw.PX.MapsTo x0 x1
+                             (ground_maps.Raw.add x l1 ((s, g0) :: g)).
+Proof.
+Admitted.
+
+Lemma setoid_list_eqk_contradiction :
+  forall l g0 s l1,
+  SetoidList.InA
+         (ground_maps.Raw.PX.eqk (elt:=list (list ground_types))) (
+         s, l1) (l) ->
+  SetoidList.NoDupA (ground_maps.Raw.PX.eqk (elt:=gt_set_type))
+         (l) ->
+  ~
+       SetoidList.InA (ground_maps.Raw.PX.eqk (elt:=gt_set_type)) (
+         s, g0) (l) ->
+  False.
+Proof.
+Admitted.
+
+Lemma ground_maps_raw_MapsTo_eq_cons :
+  forall g l0 l1 s,
+     SetoidList.NoDupA (ground_maps.Raw.PX.eqk (elt:=list (list ground_types)))
+                      ((s, l1) :: g) ->
+     ground_maps.Raw.PX.MapsTo s l0 ((s, l1) :: g) ->
+     l0 = l1.
+Proof.
+  intros. eapply ground_maps_raw_MapsTo_cons_iff in H0. destruct H0.
+  - destruct H0. eauto.
+  - unfold ground_maps.Raw.PX.MapsTo in *. pose proof (ground_maps_cons_in_contradiction).
+    specialize (H1 _ _ _ _ H0 H). contradiction.
+Qed.
+
+Lemma eqke_implies_eqk :
+  forall g s l0,
+  SetoidList.InA
+         (ground_maps.Raw.PX.eqke (elt:=list (list ground_types))) (
+           s, l0) g ->
+  SetoidList.InA
+         (ground_maps.Raw.PX.eqk (elt:=list (list ground_types))) (
+           s, l0) g.
+Proof.
+  induction g; intros.
+  - invs H.
+  - destruct a. invs H.
+    + eapply ground_maps_eqke_inversion in H1. destruct H1. subst.
+      left. reflexivity.
+    + right. eapply IHg. eauto.
+Qed.
+
+Lemma setoid_list_NoDup_eqk_fst :
+  forall g s l1 l2,
+  SetoidList.NoDupA
+    (ground_maps.Raw.PX.eqk (elt:=list (list ground_types)))
+    ((s, l1) :: g) ->
+  SetoidList.NoDupA
+    (ground_maps.Raw.PX.eqk (elt:=list (list ground_types)))
+    ((s, l2) :: g).
+Proof.
+Admitted.
+    
+Lemma ground_maps_add_Subset  :
+  forall (g1 g2: gm_type) (l1 l2: list (list ground_types)) x,
+    ground_map_Subset g1 g2 ->
+    list_set_subset l1 l2 ->
+    ground_map_Subset (ground_maps.add x l1 g1) (ground_maps.add x l2 g2).
+Proof.
+  destruct g1. rename this into g. split.
+  - revert H0. revert H. revert x. revert l1 l2. revert g2. induction g; intros.
+    + unfold ground_maps.In in *.
+      unfold ground_maps.Raw.PX.In in *.
+      destruct H1. simpl in H1. eapply ground_maps_raw_MapsTo_cons_iff in H1.
+      destruct H1; subst.
+      * destruct H1. subst. exists l2. eapply ground_maps_MapsTo_add_iff. left. eauto.
+      * invs H1.
+    + unfold ground_maps.In in *. simpl in *.
+      destruct a.
+      destruct (String_as_OT.eq_dec x s).
+      * subst. unfold ground_maps.Raw.PX.In in H1.
+        destruct H1. eapply ground_maps_raw_MapsTo_cons_iff in H1.
+        destruct H1; subst.
+        -- destruct H1; subst.
+           unfold ground_maps.Raw.PX.In. exists l2. eapply ground_maps_raw_MapsTo_add_iff. eapply (ground_maps.NoDup g2). left. eauto.
+        -- unfold ground_maps.Raw.PX.MapsTo in H1.
+           destruct (String_as_OT.eq_dec x0 s).
+           ++ subst. pose proof (ground_maps_cons_in_contradiction _ _ _ _ H1 NoDup). contradiction.
+           ++ pose proof (ground_maps_add_iff).
+              unfold ground_maps.In in H2. unfold ground_maps.add in H2. simpl in H2. destruct H.
+              eapply IHg.
+              ** split.
+                 --- intros.
+                     eapply H. unfold ground_maps.In in *. simpl. unfold ground_maps.Raw.PX.In in *. simpl in H4.
+                     destruct H4. exists x2. right. eauto.
+                 --- intros. eapply H3.
+                     eapply ground_maps.find_1. unfold ground_maps.MapsTo.
+                     eapply ground_maps.find_2 in H4.
+                     unfold ground_maps.MapsTo in H4. simpl in H4. right. eauto.
+                     eauto. eauto.
+              ** intros. eauto.
+              ** unfold ground_maps.Raw.PX.In. exists x. eapply ground_maps_raw_MapsTo_add_iff. invs NoDup. eapply H7. right. split; eauto.
+      * unfold ground_maps.Raw.PX.In in *.
+        destruct H. unfold ground_maps.In in H. unfold ground_maps.Raw.PX.In in H.
+        pose proof (ground_maps_raw_cons_add_commute).
+        destruct H1.
+        specialize (H3 _ _ _ _ _ _ _ NoDup n H1).
+        eapply ground_maps_raw_MapsTo_add_iff in H3.
+        destruct H3.
+        -- destruct H3; subst. exists l2. eapply ground_maps_raw_MapsTo_add_iff. eapply (ground_maps.NoDup g2).
+           left. eauto.
+        -- destruct H3. assert (exists e, ground_maps.Raw.PX.MapsTo x0 e ((s, g0) :: g)).
+           simpl in H.
+           exists x1. eauto.
+           eapply H in H5. destruct H5. exists x2.
+           eapply ground_maps_raw_MapsTo_add_iff. eapply (ground_maps.NoDup g2). right. split; eauto.
+        -- eauto.
+  - revert H0. revert H. revert x. revert l1 l2 g2. induction g; intros.
+    + simpl in *. unfold ground_maps.find in *.
+      eapply ground_maps.find_2 in H1, H2.
+      destruct H.
+      unfold ground_maps.MapsTo in *. simpl in *.
+      eapply ground_maps_raw_MapsTo_cons_iff in H1. destruct H1; try invs H1.
+      intros.
+      eapply ground_maps_raw_MapsTo_add_iff in H2. destruct H2.
+      destruct H2; subst. eapply H0. eauto.
+      destruct H2. congruence.
+      eapply (ground_maps.NoDup g2).
+    + pose proof (ground_maps.NoDup g2).
+      invs NoDup. destruct H.
+      eapply ground_maps.find_2 in H1.
+      destruct a.
+      destruct (String_as_OT.eq_dec x s).
+      * subst.
+        unfold ground_maps.MapsTo in *. eapply ground_maps.find_2 in H2.
+        unfold ground_maps.add in *. simpl in *.
+        destruct (String_as_OT.eq_dec s s); try congruence.
+        destruct (String_as_OT.eq_dec x0 s).
+        subst.
+        eapply ground_maps_raw_MapsTo_eq_cons in H1. subst.
+        eapply ground_maps_raw_MapsTo_add_iff in H2. destruct H2.
+        -- destruct H1. subst. eauto.
+        -- destruct H1. congruence.
+        -- eauto.
+        -- eapply setoid_list_NoDup_eqk_fst. eauto.
+        -- pose proof (ground_maps.add_3).
+           unfold ground_maps.MapsTo in H5.
+           specialize (H5 _ g2).
+           unfold ground_maps.add in H5. simpl in H5.
+           assert (s <> x0) by congruence.
+           specialize (H5 _ _ l3 l2 H8).
+           specialize (H5 H2).
+           assert (ground_maps.Raw.PX.MapsTo x0 l0 (ground_maps.Raw.add s l1 g)).
+           eapply ground_maps_raw_MapsTo_add_iff.
+           eauto.
+           invs H1.
+           eapply ground_maps_eqke_inversion in H10. destruct H10. congruence.
+           right. split; eauto.
+           eapply IHg.
+           ++ split; intros.
+              ** eapply H. unfold ground_maps.In in *. unfold ground_maps.Raw.PX.In in *.
+                 destruct H10. exists x1. right. eauto.
+              ** eapply H4. eapply ground_maps.find_1.
+                 unfold ground_maps.MapsTo. simpl.
+                 eapply ground_maps.find_2 in H10. unfold ground_maps.MapsTo in H10. simpl in H10.
+                 right. eapply H10.
+                 eauto.
+                 eauto.
+           ++ eauto.
+           ++ eapply ground_maps.find_1. eauto.
+           ++ eapply ground_maps.find_1. unfold ground_maps.MapsTo.
+              simpl. eauto.
+      * destruct (String_as_OT.eq_dec x0 x).
+        -- subst. unfold ground_maps.MapsTo in H1. simpl in H1. destruct (String_as_OT.eq_dec x s); try congruence.
+           eapply ground_maps_raw_cons_add_commute in H1.
+           pose proof (ground_maps_raw_MapsTo_add_iff).
+           specialize (H5 ((s, g0) :: g) x x l0 l1 NoDup).
+           destruct H5. specialize (H5 H1).
+           destruct H5.
+           ++ destruct H5. subst.
+              eapply IHg.
+              ** split; intros.
+                 --- eapply H. unfold ground_maps.In in *. unfold ground_maps.Raw.PX.In in *. destruct H9.
+                     destruct (String_as_OT.eq_dec x0 s).
+                     +++ subst. exists g0. simpl. eapply ground_maps_raw_MapsTo_cons_iff. left. eauto.
+                     +++ exists x1. right. eauto.
+                 --- eapply ground_maps.find_2 in H9.
+                     eapply ground_maps.find_2 in H10.
+                     unfold ground_maps.MapsTo in *.
+                     simpl in H9.
+                     eapply H4.
+                     eapply ground_maps.find_1. unfold ground_maps.MapsTo. right. eauto.
+                     eapply ground_maps.find_1. eauto.
+              ** eauto.
+              ** eapply ground_maps.find_1.
+                 eapply ground_maps.add_1. reflexivity.
+              ** eauto.
+           ++ destruct H5. congruence.
+           ++ eauto.
+           ++ eauto.
+        -- eapply H4.
+           ++ eapply ground_maps.find_1. unfold ground_maps.MapsTo in *. unfold ground_maps.add in *. simpl in *.
+              destruct (String_as_OT.eq_dec x s); try congruence.
+              eapply ground_maps_raw_MapsTo_cons_iff in H1.
+              destruct H1; subst.
+              ** destruct H1. subst.
+                 eapply ground_maps_raw_MapsTo_cons_iff. left. split; reflexivity.
+              ** eapply ground_maps_raw_MapsTo_add_iff in H1.
+                 destruct H1.
+                 destruct H1. congruence.
+                 destruct H1. right. eauto.
+                 eauto.
+           ++ eapply ground_maps.find_2 in H2.
+              eapply ground_maps_raw_MapsTo_add_iff in H2. destruct H2.
+              destruct H2. congruence.
+              destruct H2. eapply ground_maps.find_1. eauto.
+              eauto.
+              Unshelve.
+              invs NoDup. eauto.
+              invs NoDup. eauto.
+              invs NoDup. eauto.
+Qed.
