MonotoneOpSemanticsTheorems.v
@@ -1,0 +1,720 @@
+From Coq Require Import  List String Arith Psatz DecidableTypeEx OrdersEx Program.Equality FMapList FMapWeakList MSetWeakList Lists.ListSet.
+
+From VeriFGH Require Import DatalogSemantics.
+From VeriFGH Require Import OrdersFunctor DatalogProps StringOrders RelOrdered OrderedGroundTypes MoreOrders RelDecidable.
+
+Import RelSemantics.
+
+Lemma app_eq_nil {A: Type} :
+  forall (l1 l2: list A),
+    l1 ++ l2 = nil ->
+    l1 = nil /\ l2 = nil.
+Proof.
+  destruct l1; intros.
+  - simpl in H. invs H. split; reflexivity.
+  - simpl in H. inversion H.
+Qed.
+
+Lemma rev_eq_nil {A: Type}:
+  forall (l: list A),
+    rev l = nil -> l = nil.
+Proof.
+  destruct l; intros.
+  - reflexivity.
+  - simpl in H. eapply app_eq_nil in H. destruct H. congruence.
+Qed.
+
+Ltac destruct_match_goal' :=
+  match goal with
+  | [ |- ?a = match ?x with
+             | Some _ => _
+             | None => None
+             end ] =>
+      let freshX := fresh "X" in
+      destruct (x) eqn:freshX
+  end.
+
+Lemma app_cons_comm {A: Type} :
+  forall (l l': list A) (a: A),
+    l ++ a :: l' = (l ++ a :: nil) ++ l'.
+Proof.
+  induction l; simpl; intros.
+  - reflexivity.
+  - rewrite IHl. reflexivity.
+Qed.
+
+Lemma proj_tuples_fold_None :
+  forall (pvs: list string) (assoc: tup_type),
+    fold_left
+      (fun (acc : option tup_type) (elmt : string) =>
+         match assoc_lookup assoc elmt with
+         | Some gt => option_map (cons (elmt, gt)) acc
+         | None => None
+         end) pvs None = None.
+Proof.
+  induction pvs; intros.
+  - reflexivity.
+  - simpl. destruct (assoc_lookup assoc a); eapply IHpvs.
+Qed.
+
+Lemma proj_tuples_fold :
+  forall (pvs: list string) (init: tup_type) (assoc: tup_type),
+    fold_left (fun (acc: option tup_type) (elmt: string) =>
+                 match assoc_lookup assoc elmt with
+                 | Some gt => option_map (cons (elmt, gt)) acc
+                 | None => None
+                 end)
+              pvs
+              (Some init) =
+      match (fold_left (fun (acc: option tup_type) (elmt: string) =>
+                          match assoc_lookup assoc elmt with
+                          | Some gt => option_map (cons (elmt, gt)) acc
+                          | None => None
+                          end)
+                       pvs
+                       (@Some (tup_type) nil)) with
+      | Some f' => Some (f' ++ init)
+      | None => None
+      end.
+Proof.
+  induction pvs; intros.
+  - simpl. reflexivity.
+  - simpl. destruct (assoc_lookup assoc a) eqn:A.
+    + erewrite IHpvs.
+      erewrite IHpvs.
+      destruct_match_goal'.
+      * erewrite IHpvs in X.
+        symmetry. destruct_match_goal'.
+        -- destruct (fold_left
+                       (fun (acc : option tup_type) (elmt : string) =>
+                          match assoc_lookup assoc elmt with
+                          | Some gt => option_map (cons (elmt, gt)) acc
+                          | None => None
+                          end) pvs (Some nil)) eqn:X1.
+           (* Set Printing All. *)
+           unfold tup_type in X0, X1.
+           rewrite X1 in X0.
+           rewrite <- app_nil_end in X0.
+           invc X0.
+           Definition option_map_map {A' B' C': Type} (f: A' -> B' -> C') (a: option A') (b: option B') : option C' :=
+             match a, b with
+             | Some a', Some b' => Some (f a' b')
+             | _, _ => None
+             end.
+           replace (Some (t ++ init)) with (option_map_map (@app (string * ground_types)) (Some t) (Some init)) by reflexivity.
+           rewrite <- X.
+           replace ((a, g) :: init) with (((a, g) :: nil) ++ init) by reflexivity.
+           (* Set Printing All. *)
+           (* rewrite <- app_comm_cons. *)
+           (* Set Printing All. *)
+           rewrite app_assoc.
+           replace (Some ((t0 ++ (a, g) :: nil) ++ init)) with
+             (option_map_map (@app (string * ground_types))
+                             (Some ((t0 ++ (a, g) :: nil)))
+                             (Some init)) by reflexivity.
+           f_equal.
+           ++ unfold tup_type. rewrite X1. reflexivity.
+           ++ rewrite app_cons_comm.
+              f_equal. f_equal; eauto.
+              assert (Some t = Some (t0 ++ (a, g ) :: nil)).
+              rewrite <- X.
+              (* Set Printing All. *)
+              unfold tup_type in X0, X1.
+              rewrite X1 in X0.
+              inversion X0.
+              invs H.
+              reflexivity.
+        -- unfold tup_type in *.
+           destruct (fold_left
+                       (fun (acc : option (list (string * ground_types)))
+                          (elmt : string) =>
+                          match assoc_lookup assoc elmt with
+                          | Some gt => option_map (cons (elmt, gt)) acc
+                          | None => None
+                          end) pvs (Some nil)) eqn:X1.
+           inversion X0.
+           inversion X.
+      * rewrite IHpvs in X.
+        destruct (fold_left
+                    (fun (acc : option tup_type) (elmt : string) =>
+                       match assoc_lookup assoc elmt with
+                       | Some gt => option_map (cons (elmt, gt)) acc
+                       | None => None
+                       end) pvs (Some nil)) eqn:X0.
+        (* Set Printing All. *)
+        unfold tup_type in *.
+        rewrite X0.
+        rewrite X0 in X. inversion X.
+        unfold tup_type in *. rewrite X0. reflexivity.
+    + clear IHpvs. clear A.
+      revert init. revert assoc. induction pvs; intros.
+      * simpl. reflexivity.
+      * simpl.
+        destruct (assoc_lookup assoc a0).
+        -- erewrite <- IHpvs. reflexivity.
+        -- erewrite <- IHpvs. reflexivity.
+Qed.
+
+
+Lemma Some_append {A: Type} :
+  forall (l1 l2: list A),
+    Some (l1 ++ l2) = option_map_map (@app A) (Some l1) (Some l2).
+Proof.
+  intros. simpl. reflexivity.
+Qed.
+
+Lemma proj_tuples_fold_None' :
+  forall (pvs: list string) (assoc init: tup_type),
+    fold_left
+      (fun (acc : option (list (string * ground_types))) (elmt : string)
+       =>
+         match assoc_lookup assoc elmt with
+         | Some gt => option_map (cons (elmt, gt)) acc
+         | None => None
+         end) pvs (Some init) = None ->
+    proj_tuples pvs assoc = None.
+Proof.
+  induction pvs; intros.
+  - simpl in H. inversion H.
+  - simpl. simpl in H.
+    destruct (assoc_lookup assoc a) eqn:A.
+    + eapply IHpvs in H.
+      rewrite proj_tuples_fold.
+      simpl in H. unfold tup_type in *. rewrite H. reflexivity.
+    + rewrite proj_tuples_fold_None. reflexivity.
+Qed.
+
+
+Lemma proj_tuples_append :
+  forall (pvs pvs': list string) (s: string) (g: ground_types) (res res' assoc: tup_type),
+    proj_tuples (pvs ++ pvs') assoc =
+      match (proj_tuples pvs assoc), proj_tuples pvs' assoc with
+      | Some res, Some res' =>
+          Some (res' ++ res)
+      | _, _ => None
+      end.
+Proof.
+  induction pvs; intros.
+  - simpl. destruct_match_goal'.
+    + rewrite <- app_nil_end. reflexivity.
+    + reflexivity.
+  - destruct (proj_tuples (a :: pvs) assoc) eqn:X.
+    + rewrite <- app_nil_l with (l := pvs) in X.
+      rewrite app_comm_cons in X.
+      specialize (IHpvs pvs').
+      specialize (IHpvs s g res res' assoc).
+      destruct (proj_tuples pvs' assoc) eqn:P.
+      * destruct (proj_tuples pvs assoc) eqn:P'.
+        -- simpl. simpl in X. destruct (assoc_lookup assoc a) eqn:A.
+           ++ rewrite proj_tuples_fold.
+              rewrite proj_tuples_fold in X.
+              unfold tup_type in *.
+              replace (fold_left
+                         (fun (acc : option (list (string * ground_types))) (elmt : string) =>
+                            match assoc_lookup assoc elmt with
+                            | Some gt => option_map (cons (elmt, gt)) acc
+                            | None => None
+                            end) (pvs ++ pvs') (Some nil)) with (proj_tuples (pvs ++ pvs') assoc) by reflexivity.
+              rewrite IHpvs.
+              
+              rewrite <- app_assoc.
+              rewrite Some_append.
+              rewrite Some_append at 1.
+              rewrite Some_append.
+              f_equal.
+              simpl. rewrite <- X.
+              destruct_match_goal'.
+              replace (fold_left
+                         (fun (acc : option (list (string * ground_types)))
+                            (elmt : string) =>
+                            match assoc_lookup assoc elmt with
+                            | Some gt => option_map (cons (elmt, gt)) acc
+                            | None => None
+                            end) pvs (Some nil)) with (proj_tuples pvs assoc) in X0 by reflexivity.
+              rewrite X0 in P'. invs P'. reflexivity.
+              inversion X.
+           ++ rewrite proj_tuples_fold_None in X. inversion X.
+        -- simpl in X.
+           destruct (assoc_lookup assoc a) eqn:A.
+           ++ rewrite proj_tuples_fold in X.
+              simpl in P'. unfold tup_type in *. rewrite P' in X. inversion X.
+           ++ rewrite proj_tuples_fold_None in X. inversion X.
+      * simpl in X. pose proof (PROJ := proj_tuples_fold).
+        unfold tup_type in *.
+        destruct (assoc_lookup assoc a) eqn:A.
+        rewrite PROJ in X.
+        fold (proj_tuples pvs assoc) in X.
+        destruct (proj_tuples pvs assoc).
+        simpl. rewrite A.
+        rewrite proj_tuples_fold.
+        simpl in IHpvs.
+        unfold tup_type in *. rewrite IHpvs. reflexivity.
+        inversion X.
+        rewrite proj_tuples_fold_None in X. invs X.
+    + simpl. destruct (assoc_lookup assoc a) eqn:A.
+      * rewrite proj_tuples_fold.
+        unfold proj_tuples in *. unfold tup_type in *. rewrite IHpvs.
+        simpl in X.
+        rewrite A in X.
+        pose proof (PROJ := proj_tuples_fold_None').
+        unfold tup_type in *. simpl in PROJ. erewrite PROJ. reflexivity.
+        eapply proj_tuples_fold_None' in X.
+        simpl in X. unfold tup_type in *. rewrite X. reflexivity.
+        eassumption. eassumption.
+        eassumption. eassumption.
+      * rewrite proj_tuples_fold_None. reflexivity.
+Qed.
+
+
+
+
+
+
+
+Lemma proj_tuples_cons :
+  forall (pvs: list string) (s: string) (g: ground_types) (res assoc: tup_type),
+    proj_tuples (s :: pvs) assoc =
+      match (proj_tuples pvs assoc), assoc_lookup assoc s with
+      | Some res, Some g =>
+          Some (res ++ ((s, g) :: nil))
+      | _, _ => None
+      end.
+Proof.
+  intros.
+  replace (s :: pvs) with ((s :: nil) ++ pvs) by reflexivity.
+  rewrite proj_tuples_append; try eassumption.
+  destruct (proj_tuples (s :: nil) assoc) eqn:P.
+  - destruct (proj_tuples pvs assoc) eqn:P'.
+    + simpl in P. destruct (assoc_lookup assoc s) eqn:A.
+      * invs P. reflexivity.
+      * invs P.
+    + reflexivity.
+  - simpl in P. destruct (assoc_lookup assoc s). inversion P.
+    destruct (proj_tuples pvs assoc); reflexivity.
+Qed.
+
+
+
+Lemma proj_tuples_adequacy :
+  forall (pvs: list string) (assoc tt: tup_type),
+    proj_tuples_rel pvs assoc tt <->
+      Some (rev tt) = proj_tuples pvs assoc.
+Proof.
+  induction pvs; intros; split; intros.
+  - invs H. simpl. reflexivity.
+  - simpl in H. invs H.
+    destruct tt; invs H1.
+    econstructor.
+    eapply app_eq_nil in H2. destruct H2. inversion H2.
+    
+  - invs H. eapply IHpvs in H5. simpl.
+    eapply assoc_lookup_adequacy in H2.
+    rewrite <- H2. 
+    match goal with
+    | [ |- @Some ?tipe ?x = _ ] =>
+        replace (@Some tipe x) with (option_map_map (@app (string * ground_types)) (Some (rev res)) ((Some ((a, g) :: nil)))) by reflexivity
+    end.
+    rewrite H5.
+    pose proof (proj_tuples_append).
+    specialize (H0 (a :: nil) pvs).
+    specialize (H0 a g assoc res assoc).
+    simpl in H0.
+    rewrite <- H2 in H0.
+    rewrite H0. simpl.
+    rewrite <- H0. unfold option_map_map.
+    symmetry.
+    destruct_match_goal'.
+    + eassumption.
+    + eassumption.
+  - simpl in H. destruct (assoc_lookup assoc a) eqn:A.
+    + rewrite proj_tuples_fold in H.
+      unfold tup_type in *.
+      replace (fold_left (fun (acc : option (list (string * ground_types))) (elmt : string) =>
+                            match assoc_lookup assoc elmt with
+                            | Some gt => option_map (cons (elmt, gt)) acc
+                            | None => None
+                            end) pvs (Some nil)) with (proj_tuples pvs assoc) in H by reflexivity.
+      destruct (proj_tuples pvs assoc) eqn:P.
+      * invs H.
+        assert (rev (rev tt) = (rev (l ++ (a, g) :: nil))) by (f_equal; eauto).
+        rewrite rev_involutive in H0. rewrite H0.
+        rewrite rev_app_distr.
+        simpl. econstructor.
+        eapply assoc_lookup_adequacy. congruence.
+        eapply IHpvs.
+        rewrite rev_involutive. congruence.
+      * invs H.
+    + rewrite proj_tuples_fold_None in H. invs H.
+Qed.
+
+Lemma set_inter_subset_empty :
+  forall v' a init,
+    set_inter str_gt_list_ot.eq_dec (a :: v') init =
+      empty_set str_gt_list_ot.t ->
+    set_inter str_gt_list_ot.eq_dec v' init =
+      empty_set str_gt_list_ot.t.
+Proof.
+  induction v'; intros.
+  - reflexivity.
+  - simpl in H. destruct (set_mem str_gt_list_ot.eq_dec a0 init) eqn:A0; try congruence.
+    + inversion H.
+    + destruct (set_mem str_gt_list_ot.eq_dec a init) eqn:A; try congruence.
+      * inversion H.
+      * simpl.
+        rewrite A. eassumption.
+Qed.
+
+
+(* Lemma set_inter_comm {A: Type} : *)
+(*   forall (Aeq_dec: forall (a1 a2: A), {a1 = a2} + {a1 <> a2}) a b, *)
+(*     set_inter Aeq_dec a b = set_inter Aeq_dec b a. *)
+(* Proof. *)
+(*   induction a; intros. *)
+(*   - induction b; eauto. *)
+(*   - induction b. simpl. rewrite IHa. reflexivity. *)
+(*     simpl; destruct (set_mem Aeq_dec a b) eqn:S. *)
+(*     +  *)
+(*       destruct (Aeq_dec a a1); destruct (Aeq_dec a1 a); try congruence. *)
+(*       * subst. rewrite <- IHb. *)
+(*         f_equal. *)
+(*         eapply list_set_equality. *)
+(*         simpl. intros; split; intros. *)
+(*         -- destruct (set_mem Aeq_dec a1 b). *)
+(*            ++ rewrite IHa in H. simpl in H. *)
+(*               destruct (set_mem Aeq_dec a1 a0) eqn:A'. *)
+(*               ** rewrite <- IHa in H. eassumption. *)
+(*               ** rewrite <- IHa in H. *)
+(*                  unfold set_In in *. *)
+(*                  simpl. right. eassumption. *)
+(*            ++ inversion S. *)
+(*         -- rewrite S in H. simpl in IHb. rewrite S in IHb. rewrite IHb in H. *)
+(*            rewrite IHa. simpl. destruct (set_mem Aeq_dec a1 a0) eqn:A'. *)
+(*            ++ rewrite <- IHb in H. rewrite IHa in H. eassumption. *)
+(*            ++ rewrite <- IHb in H. simpl in H. destruct H. *)
+(*               ** subst. *)
+(*         simpl. symmetry. *)
+(*         rewrite S. *)
+(*         symmetry. rewrite IHa. *)
+(*         simpl. *)
+(*         symmetry. *)
+
+
+(*       revert S. *)
+
+
+
+(*       * simpl. inversion S. *)
+(*       * simpl in S. *)
+(*         destruct (Aeq_dec a a1) eqn:A1. *)
+(*         -- subst. simpl. rewrite A1. *)
+
+
+
+Lemma set_inter_elements {A: Type} :
+  forall (Aeq_dec : forall (a1 a2: A), { a1 = a2 } + { a1 <> a2 }) l1 l2 a,
+    set_In a (set_inter Aeq_dec l1 l2) <->
+      set_In a l1 /\ set_In a l2.
+Proof.
+  induction l1; intros; split; intros.
+  - simpl in H. inversion H.
+  - destruct H. invs H.
+  - simpl in H. destruct (set_mem Aeq_dec a l2) eqn:A'.
+    + eapply set_mem_correct1 in A'.
+      simpl in H. destruct H.
+      * subst. split.
+        -- simpl. left. reflexivity.
+        -- eassumption.
+      * eapply IHl1 in H. destruct H.
+        split; simpl.
+        -- right. eassumption.
+        -- eassumption.
+    + eapply IHl1 in H. destruct H. split; simpl.
+      * right. eassumption.
+      * eassumption.
+  - simpl in H. destruct H.
+    destruct H.
+    + simpl. subst. eapply set_mem_correct2 in H0. erewrite H0.
+      simpl. left. reflexivity.
+    + simpl. destruct (set_mem Aeq_dec a l2) eqn:A'.
+      * simpl. right. eapply IHl1; eauto.
+      * eapply IHl1; eauto.
+Qed.
+
+
+
+Lemma set_inter_empty :
+  forall v' a init,
+    set_inter str_gt_list_ot.eq_dec v' (a :: init) =
+      empty_set str_gt_list_ot.t ->
+    ~ (set_In a v').
+Proof.
+  induction v'; intros.
+  - unfold not; intros. inversion H0.
+  - simpl. unfold not. intros.
+    destruct H0.
+    + subst. simpl in H.
+      destruct (str_gt_list_ot.eq_dec a0 a0); try congruence.
+      invs H.
+    + eapply set_inter_subset_empty in H.
+      assert (set_In a0 (a0 :: init)).
+      {
+        simpl. left. reflexivity.
+      }
+      assert (set_In a0 (set_inter str_gt_list_ot.eq_dec v' (a0 :: init))).
+      {
+        eapply set_inter_elements; split; eauto.
+      }
+      rewrite H in H2. invs H2.
+Qed.
+
+
+
+Lemma proj_relation_init :
+  forall (init v: tup_set) (pvs: list string) v' a l,
+    Some v' = proj_relation pvs (a :: v) ->
+    set_inter str_gt_list_ot.eq_dec v' init =
+      empty_set str_gt_list_ot.t ->
+    proj_tuples pvs a = Some l ->
+    init ++ l :: nil = set_add str_gt_list_ot.eq_dec l init.
+Proof.
+  induction init; intros; simpl.
+  - reflexivity.
+  - destruct (str_gt_list_ot.eq_dec l a).
+    + eapply set_inter_empty in H0.
+      unfold str_gt_list_ot.eq in e.
+      subst.
+      Opaque proj_tuples.
+      simpl in H.
+      rewrite H1 in H.
+      eapply list_set_equality.
+      simpl. intros.
+      split; intros.
+      * pose proof (str_gt_list_ot.eq_dec a x). destruct H3.
+        -- destruct H2.
+           ++ left. eassumption.
+           ++ invs e. left. reflexivity.
+        -- destruct H2. congruence.
+           right. eapply in_app_or in H2.
+           destruct H2.
+           ++ eassumption.
+           ++ simpl in H2. destruct H2; try congruence.
+              contradiction.
+      * destruct H2.
+        -- left. eauto.
+        -- right. eapply in_or_app. left. eauto.
+    + erewrite IHinit; eauto.
+      pose proof (set_inter_empty).
+      specialize (H2 v' a init).
+      specialize (H2 H0).
+      eapply list_set_equality.
+      simpl. intros. split; intros.
+      * eapply set_inter_elements in H3. destruct H3.
+        assert (set_In x (a :: init)).
+        {
+          simpl. right. eassumption.
+        }
+        pose proof (@set_inter_elements tup_type).
+        specialize (H6 str_gt_list_ot.eq_dec v' (a :: init)).
+        specialize (H6 x). destruct H6.
+        assert (set_In x v' /\ set_In x (a :: init)) by (split; eauto).
+        eapply H7 in H8.
+        (* Set Printing All. *)
+        unfold str_gt_list_ot.t in *. unfold tup_type in *.
+        rewrite H0 in H8.
+        inversion H8.
+      * inversion H3.
+Qed.
+
+Lemma proj_relation_fold :
+  forall (v v' init: tup_set) (pvs: list string),
+    Some v' = proj_relation pvs v ->
+    set_inter (str_gt_list_ot.eq_dec) v' init = empty_set str_gt_list_ot.t ->
+    set_fold_left (fun (acc : option (set tup_type)) (elmt : tup_type) =>
+                     match proj_tuples pvs elmt with
+                     | Some tup => option_map (set_add str_gt_list_ot.eq_dec tup) acc
+                     | None => None
+                     end) v (Some (init)) =
+      match set_fold_left (fun (acc : option (set tup_type)) (elmt : tup_type) =>
+                             match proj_tuples pvs elmt with
+                             | Some tup => option_map (set_add str_gt_list_ot.eq_dec tup) acc
+                             | None => None
+                             end) v (Some (empty_set tup_type)) with
+      | Some f' => Some (init ++ f')
+      | None => None
+      end.
+Proof.
+  induction v; intros.
+  - simpl. unfold empty_set. rewrite app_nil_r. reflexivity.
+  - Opaque proj_tuples. simpl.
+    destruct (proj_tuples pvs a) eqn:P.
+    + pose proof (PJ := H). simpl in H. rewrite P in H.
+      unfold tup_type in *.
+      destruct (proj_relation pvs v) eqn:J.
+      * erewrite IHv in H.
+        -- simpl in J. unfold tup_type in *. rewrite J in H.
+           erewrite IHv.
+           erewrite IHv.
+           rewrite J. erewrite IHv. rewrite J.
+           simpl. f_equal.
+           eapply list_set_equality.
+           simpl. intros; split; intros.
+           eapply in_app_or in H1.
+           destruct H1.
+           ++ eapply set_add_elim in H1. destruct H1.
+              eapply in_or_app. right. simpl. left. congruence.
+              eapply in_or_app. left. eassumption.
+           ++ eapply in_or_app. right. simpl. right. eassumption.
+           ++ eapply in_or_app.
+              eapply in_app_or in H1. destruct H1.
+              ** left. eapply set_add_intro1.
+                 eassumption.
+              ** simpl in H1. destruct H1.
+                 --- subst. left. eapply set_add_intro2. reflexivity.
+                 --- right. eassumption.
+           ++ simpl.
+Admitted.
+(*      erewrite <- proj_relation_init. *)
+(*      rewrite <- app_assoc. simpl. reflexivity. *)
+(*      eassumption. *)
+(*      eassumption. *)
+(*      eassumption. *)
+(*      symmetry. eauto. *)
+
+
+
+(* erewrite IHv. *)
+(* symmetry. erewrite IHv. symmetry. *)
+(* symmetry. destruct_match_goal'. *)
+(* * rewrite app_assoc. f_equal. f_equal. *)
+(*   eapply proj_relation_init. eassumption. eassumption. *)
+(*   eassumption. *)
+(* * reflexivity. *)
+(* * simpl in H. rewrite P in H. erewrite IHv in H; eauto. *)
+(*   fold (proj_relation pvs v) in H. *)
+(*   destruct (proj_relation pvs v).  *)
+
+
+Lemma proj_relation_adequacy :
+  forall (t1 t2: tup_set)  (pvs: list string),
+    proj_relation_rel pvs t1 t2 <->
+      Some (rev (map (@rev (string * ground_types)) t2)) = proj_relation pvs t1.
+Proof.
+  induction t1; intros; split; intros.
+  - inversion H. simpl. reflexivity.
+  - simpl in H. invs H. unfold empty_set in H1.
+    eapply rev_eq_nil in H1.
+    destruct t2. simpl in H1. econstructor.
+    simpl in H1. invs H1.
+  - invs H.
+    eapply IHt1 in H5.
+    remember (proj_relation pvs (a :: t1)) as temp.
+    simpl. subst.
+    rewrite Some_append. rewrite H5.
+    eapply proj_tuples_adequacy in H3.
+    Opaque proj_tuples.
+    simpl.
+    rewrite <- H3.
+    unfold set_fold_left.
+    unfold empty_set.
+    
+    (* rewrit *)
+
+Admitted.
+
+Lemma monotone_op_semantics_det :
+    forall (m: monotone_ops) (g: gm_type) (v v': ListSet.set tup_type),
+      monotone_op_semantics g m v ->
+      monotone_op_semantics g m v' ->
+      v = v'.
+  Proof.
+    induction m; intros.
+    - inversion H.
+    - inversion H. inversion H0. subst.
+      rewrite H7 in H3. inversion H3. reflexivity.
+    - inversion H. inversion H0. subst.
+      f_equal. eapply IHm; eassumption.
+    - inversion H. inversion H0. subst. f_equal; eauto.
+    - inversion H. inversion H0. subst.
+      specialize (IHm _ _ _ H4 H10). subst. rewrite H12 in H6. inversion H6. reflexivity.
+    - inversion H. inversion H0. subst.
+      f_equal; eauto.
+  Qed.
+
+  Lemma monotone_op_semantics_adequacy :
+    forall (m: monotone_ops) (g: gm_type) (v: ListSet.set tup_type),
+      Some v = monotone_op_semantics_eval g m <->
+        monotone_op_semantics g m v.
+  Proof.
+    induction m; intros; split; intros.
+    - simpl in H. inversion H.
+    - inversion H.
+    - simpl in H.
+      match goal with
+      | [ H: Some _ = match ?x with | Some v => _ | None => None end |- _ ] =>
+          destruct (x) eqn:X; inversion H
+      end.
+      econstructor. eassumption.
+    - inversion H. simpl. rewrite H2. reflexivity.
+    - simpl in H.
+      Ltac destruct_hyp_match :=
+        match goal with
+        | [H: Some _ = match ?x with | Some _ => _ | None => None end |- _ ] =>
+            let Xfresh := fresh "X" in
+            destruct (x) eqn:Xfresh; inversion H
+        end.
+      destruct_hyp_match.
+      symmetry in X. eapply IHm in X.
+      econstructor; eauto.
+    - Ltac destruct_goal_match :=
+        match goal with
+        | [ |- Some _ = match ?x with | Some _ => _ | None => None end ] =>
+            let Xfresh := fresh "X" in
+            destruct (x) eqn:Xfresh; subst
+        end.
+      simpl. destruct_goal_match.
+      + inversion H. subst. eapply IHm in H5.
+        rewrite <- H5 in X. inversion X. reflexivity.
+      + inversion H. subst. eapply IHm in H5. rewrite X in H5. congruence.
+    - simpl in H.
+      match goal with
+      | [H: Some _ = match ?x with | Some _ => _ | None => None end |- _ ] =>
+          destruct (x) eqn:X; inversion H
+      end.
+      
+      destruct_hyp_match.
+      subst.
+      econstructor; eauto.
+      eapply IHm1. congruence.
+      eapply IHm2. congruence.
+    - inversion H. subst. simpl.
+      
+
+      destruct_goal_match.
+      + destruct_goal_match.
+        * f_equal. eapply IHm1 in H2. eapply IHm2 in H4.
+          rewrite <- H2 in X. rewrite <- H4 in X0.
+          inversion X. inversion X0. reflexivity.
+        * eapply IHm2 in H4. rewrite <- H4 in X0. inversion X0.
+      + eapply IHm1 in H2. rewrite <- H2 in X. inversion X.
+    - simpl in H. destruct_hyp_match.
+      econstructor. eapply IHm. symmetry. eassumption. simpl. 
+      congruence.
+    - simpl. inversion H. subst. destruct_goal_match.
+      symmetry in X.
+      eapply IHm in X.
+      pose proof (monotone_op_semantics_det _ _ _ _ H3 X). subst.
+      simpl in *.
+      congruence.
+      eapply IHm in H3. rewrite X in H3. congruence.
+    - simpl in H. destruct_hyp_match. destruct_hyp_match.
+      econstructor; eauto.
+      eapply IHm1.
+  Admitted.
+  (* congruence. *)
+      (* eapply IHm2. congruence. *)
+    (* - inversion H. subst. eapply IHm1 in H4. eapply IHm2 in H6. *)
+      (* simpl. rewrite <- H4. rewrite <- H6. reflexivity. *)
+  (* Qed. *)
+
+  
+  (* Eval compute in ground_maps.t. *)
