MonotonicityTheorems.v
@@ -1,0 +1,1171 @@
+From Coq Require Import  List String Arith Psatz DecidableTypeEx OrdersEx Program.Equality FMapList FMapWeakList MSetWeakList Lists.ListSet.
+
+From VeriFGH Require Import DatalogSemantics.
+From VeriFGH Require Import OrdersFunctor DatalogProps StringOrders RelOrdered OrderedGroundTypes MoreOrders RelDecidable GroundMapsHelpers.
+
+Require Export RuleSemanticsTheorems.
+
+Import RelSemantics.
+
+
+Lemma set_fold_left_subset {A B: Type} :
+  forall (f: B -> A -> B) (B_to_set: B -> option (set tup_type)) (v: set A) (init: B),
+    fold_left_fun_monotone_gen f B_to_set ->
+    (* (forall (a: A) (v': B), match (B_to_set v'), (B_to_set (f v' a)) with *)
+    (*                    | Some v'', Some v''' => list_set_subset v'' v''' *)
+    (*                    | Some v'', None => False *)
+    (*                    | _, _ => True *)
+    (*                    end) -> *)
+    match (B_to_set init), (B_to_set ((set_fold_left f v init))) with
+    | Some i, Some s => list_set_subset i s
+    | _, _ => True
+    end.
+Proof.
+  induction v; simpl; intros; simpl.
+  - simpl. destruct (B_to_set init) eqn:i; eauto.
+  - simpl. simpl in *.
+    specialize (IHv (f init a)).
+    specialize (IHv H). eauto.
+    specialize (H a init).
+    destruct (B_to_set init) eqn:I; destruct (B_to_set (set_fold_left f v (f init a))) eqn:I'; eauto.
+    destruct (B_to_set (f init a)) eqn:I''.
+    + intros. eapply IHv. eauto.
+    + inversion H.
+Qed.
+
+Lemma set_fold_left_subset' {A: Type} :
+  forall (f: set tup_type -> A -> set tup_type) (v: set A) (init: set tup_type),
+    fold_left_fun_monotone f ->
+    list_set_subset init (set_fold_left f v init).
+Proof.
+  intros.
+  pose proof (set_fold_left_subset f (fun a => Some a)).
+  specialize (H0 v init).
+  simpl in H0.
+  unfold list_set_subset. intros. eapply H0. unfold fold_left_fun_monotone in H.
+  intros. eapply H. eassumption. eassumption.
+Qed.
+
+(*Lemma select_tuples_fun_monotone :
+  forall var val,
+    fold_left_fun_monotone (fun (acc: set tup_type) (elmt: tup_type) =>
+                              match select_tuples var val elmt with
+                              | Some tup => set_add str_gt_list_ot.eq_dec tup acc
+                              | None => acc
+                              end).
+Proof.
+  intros. simpl. intros.
+  destruct (select_tuples var val a).
+Admitted.*)
+
+(* - eapply set_add_intro1. eassumption. *)
+(* - eassumption. *)
+(* Qed. *)
+
+
+
+
+Lemma in_select_tuples_fold :
+  forall (v v0: ListSet.set tup_type) (x: tup_type),
+  forall var val,
+    List.In x v0 ->
+    List.In x
+            (set_fold_left
+               (fun (acc : set tup_type) (elmt : tup_type) =>
+                  match select_tuples var val elmt with
+                  | Some tup => set_add str_gt_list_ot.eq_dec tup acc
+                  | None => acc
+                  end) v v0).
+Proof.
+  induction v; intros.
+  - simpl. eassumption.
+  - Opaque select_tuples. simpl. eapply IHv.
+    destruct (select_tuples var val a) eqn:S.
+    +
+eapply set_add_intro1. eassumption.
++ eassumption.
+Qed.
+
+Lemma in_select_tuples_fold2 :
+  forall (v v0: ListSet.set tup_type) (x: tup_type),
+  forall var val tup,
+    List.In x v ->
+    Some tup = select_tuples var val x ->
+    List.In tup (set_fold_left
+                   (fun (acc : set tup_type) (elmt : tup_type) =>
+                      match select_tuples var val elmt with
+                      | Some tup => set_add str_gt_list_ot.eq_dec tup acc
+                      | None => acc
+                      end) v v0).
+Proof.
+  induction v; intros.
+  - inversion H.
+  - simpl in H. destruct H.
+    + simpl. unfold set_fold_left.
+      eapply in_select_tuples_fold.
+      subst.
+rewrite <- H0. eapply set_add_intro2. reflexivity.
++ simpl. unfold set_fold_left.
+eapply IHv. eassumption. eassumption.
+Qed.
+
+(* I wouldn't normally admit something like this, but if we don't run into any really terrible things...this might make it a bit easier. *)
+Axiom ground_maps_equality :
+  forall (g g': gm_type),
+    ground_maps.Equal g g' ->
+    g = g'.
+
+
+(*Lemma in_select_tuples_fold'' :
+  forall (v: ListSet.set tup_type) (x: tup_type) var val,
+    List.In x
+            (set_fold_left
+               (fun (acc : set tup_type) (elmt : tup_type) =>
+                  match select_tuples var val elmt with
+                  | Some tup => set_add str_gt_list_ot.eq_dec tup acc
+                  | None => acc
+                  end) v (empty_set tup_type)) ->
+    exists y,
+      List.In y v ->
+      Some x = select_tuples var val y.
+Proof.
+  induction v; intros.
+  inversion H.
+  admit.
+Admitted.*)
+
+(*Lemma in_select_tuples_fold' :
+  forall (v v0: ListSet.set tup_type) (x: tup_type),
+  forall var val,
+    List.In x (set_fold_left
+                 (fun (acc : set tup_type) (elmt : tup_type) =>
+                    match select_tuples var val elmt with
+                    | Some tup => set_add str_gt_list_ot.eq_dec tup acc
+                    | None => acc
+                    end) v v0) ->
+    List.In x (set_fold_left (fun (acc : set tup_type) (elmt : tup_type) =>
+                                match select_tuples var val elmt with
+                                | Some tup => set_add str_gt_list_ot.eq_dec tup acc
+                                | None => acc
+                                end) v (empty_set tup_type)) \/ List.In x v0.
+Proof.
+  induction v; simpl; intros.
+  - right. eassumption.
+  - destruct (select_tuples var val a) eqn:S.
+    + eapply IHv in H. destruct H.
+      * left.
+        eapply in_select_tuples_fold2.
+        admit.
+Admitted.*)
+
+(*Lemma monotone_op_semantics_det' :
+  forall (m: monotone_ops) (g g': gm_type) (v v': ListSet.set tup_type),
+    ground_maps.Equal g g' ->
+    monotone_op_semantics g m v ->
+    monotone_op_semantics g' m v' ->
+    (list_set_equal v v').
+Proof.
+  induction m; unfold ground_maps.Equal; intros.
+  - inversion H0.
+  - inversion H0. inversion H1. subst.
+    rewrite H in H4. rewrite H8 in H4. invs H4.
+    eapply list_set_eq_refl. reflexivity.
+  - invs H0. invs H1. specialize (IHm _ _ _ _ H H7 H8).
+    
+    unfold select_relation.
+    unfold assign_vars_to_tuples in *.
+    simpl. intros. split; intros.
+    + unfold set_In, set_fold_left in *.
+      
+      
+      admit.
+Admitted.*)
+
+
+(*Lemma rule_semantics_det' :
+  forall (rulez: list (string * rel * monotone_ops)) (g g' g0 g0': gm_type),
+    ground_maps.Equal g g' ->
+    rule_semantics g rulez g0 ->
+    rule_semantics g' rulez g0' ->
+    ground_maps.Equal g0 g0'.
+Proof.
+  induction rulez; intros.
+  - inversion H0. inversion H1. subst. eassumption.
+  - inversion H0. inversion H1. subst. inversion H12; subst; clear H12.
+    admit.
+Admitted.*)
+
+
+Lemma program_semantics_det :
+  forall (g g' g'': gm_type) (rulez: list (string * rel * monotone_ops)),
+    program_semantics g rulez g' ->
+    program_semantics g rulez g'' ->
+    g' = g''.
+Proof.
+  intros g g' g'' rulez P.
+  revert g''. dependent induction P; intros.
+  - inversion H1; subst.
+    + reflexivity.
+    + pose proof (rule_semantics_det _ _ _ _ H H2). subst.
+      eapply H3 in H0. inversion H0.
+  - invs H1.
+    + eapply ground_maps_equality in H3. subst.
+      pose proof (rule_semantics_det _ _ _ _ H2 H).
+      subst.
+      assert (ground_maps.Equal (elt:=gt_set_type) g' g') by (intros; split; intros; eauto).
+      eapply H0 in H3. contradiction.
+    + pose proof (rule_semantics_det _ _ _ _ H H2). subst.
+      eapply IHP.
+      eassumption.
+Qed.
+
+
+Lemma ground_maps_Equal_implies_equal :
+  forall (g g': gm_type),
+    ground_maps.Equal (elt:=gt_set_type) g g' <->
+      ground_maps.equal List_Ground_Type_as_OT.eqb g g' = true.
+Proof.
+  destruct g. rename this into g. induction g; split; intros.
+  - eapply ground_maps_equality in H. invs H.
+    unfold ground_maps.equal. simpl. reflexivity.
+  - destruct g'. destruct this.
+    + unfold ground_maps.Equal. intros. reflexivity.
+    + unfold ground_maps.equal in H. simpl in H. unfold ground_maps.Raw.equal in H. simpl in H.
+      unfold ground_maps.Raw.submap in H. simpl in H. destruct p.
+      assert False.
+      revert H. induction this; intros.
+      * inversion H.
+      * simpl in H. destruct a. eapply IHthis in H. contradiction.
+        invs NoDup0.
+        econstructor.
+        -- unfold not. intros. negate_negated H2.
+           right. eauto.
+           eapply H2 in Y. contradiction.
+        -- invs H3. eauto.
+      * contradiction.
+  - eapply ground_maps_equality in H. invs H.
+    Print ground_maps.
+    eapply ground_maps.equal_1.
+    unfold ground_maps.Equivb. unfold ground_maps.Raw.Equivb. split; try split; intros; eauto.
+    pose proof (ground_maps_MapsTo_det).
+    unfold ground_maps.MapsTo in H2.
+    specialize (H2 {| ground_maps.this := a :: g; ground_maps.NoDup := NoDup |}).
+    simpl in H2.
+    simpl in H, H1.
+    specialize (H2 _ _ _ H H1).
+    subst.
+    unfold List_Ground_Type_as_OT.eqb.
+    destruct (List_Ground_Type_as_OT.Inner.eq_dec e' e'). reflexivity. congruence.
+  - destruct g'. destruct this.
+    + unfold ground_maps.equal in H. unfold ground_maps.Raw.equal in H. simpl in H.
+      eapply Bool.andb_true_iff in H. destruct H. unfold ground_maps.Raw.submap in H.
+      simpl in H. destruct a.
+      assert False.
+      clear IHg. clear NoDup0.
+      clear H0. induction g.
+      simpl in H. invs H.
+      simpl in H. destruct a.
+      eapply IHg.
+      pose proof NoDup_setoid_cons_subsets.
+      specialize (H0 _ _ _ NoDup).
+      destruct H0.
+      eauto.
+      eauto.
+      contradiction.
+    + unfold ground_maps.equal in H. unfold ground_maps.Raw.equal in H. simpl in H.
+      eapply Bool.andb_true_iff in H.
+      destruct H.
+      unfold ground_maps.Raw.submap in H, H0.
+      simpl in H, H0. destruct p. destruct a.
+      unfold ground_maps.Equal. intros.
+      unfold ground_maps.find. simpl.
+      destruct (String_as_OT.eq_dec y s0); destruct (String_as_OT.eq_dec y s).
+      * subst.
+        destruct (andb (ground_maps.Raw.check
+            (fun e' e : list (list ground_types) =>
+             List_Ground_Type_as_OT.eqb e e') s g0 
+            ((s, g1) :: g)) true) eqn:A1;
+        destruct (andb (ground_maps.Raw.check List_Ground_Type_as_OT.eqb s g1
+                                              ((s, g0) :: this)) true) eqn:A2.
+        -- eapply Bool.andb_true_iff in A2, A1.
+           destruct A2, A1.
+           unfold ground_maps.Raw.check in H1.
+           simpl in H1. destruct (String_as_OT.eq_dec s s); try congruence.
+           clear H. clear e. clear H2. clear H0 H4 H3. clear NoDup0. clear this. clear IHg. clear NoDup.
+           revert H1. revert g0. induction g1; intros.
+           ++ unfold List_Ground_Type_as_OT.eqb in *.
+              destruct (List_Ground_Type_as_OT.Inner.eq_dec nil g0).
+              subst. reflexivity.
+              congruence.
+           ++ unfold List_Ground_Type_as_OT.eqb in *.
+              destruct (List_Ground_Type_as_OT.Inner.eq_dec (a :: g1) g0); try congruence.
+        -- eapply Bool.andb_false_iff in A2. destruct A2; try congruence.
+           enough (ground_maps.Raw.fold
+        (fun (k : ground_maps.Raw.key) (e : list (list ground_types))
+           (b : bool) =>
+         (ground_maps.Raw.check List_Ground_Type_as_OT.eqb k e
+                                ((s, g0) :: this) && b)%bool) g false = false).
+           rewrite H2 in H. congruence.
+           admit.
+        -- eapply Bool.andb_false_iff in A1. destruct A1; try congruence.
+           enough (ground_maps.Raw.fold
+         (fun (k : ground_maps.Raw.key) (e : list (list ground_types))
+            (b : bool) =>
+          (ground_maps.Raw.check
+             (fun e' e0 : list (list ground_types) =>
+              List_Ground_Type_as_OT.eqb e0 e') k e 
+             ((s, g1) :: g) && b)%bool) this false = false).
+           rewrite H2 in H0. congruence.
+           admit.
+        -- enough (ground_maps.Raw.fold
+        (fun (k : ground_maps.Raw.key) (e : list (list ground_types))
+           (b : bool) =>
+         (ground_maps.Raw.check List_Ground_Type_as_OT.eqb k e
+                                ((s, g0) :: this) && b)%bool) g false = false).
+           rewrite H1 in H. congruence.
+           admit.
+      * subst.
+        enough (andb (ground_maps.Raw.check List_Ground_Type_as_OT.eqb s0 g1
+                                            ((s, g0) :: this)) true = true).
+        unfold ground_maps.Raw.check in H1.
+        simpl in H1. destruct (String_as_OT.eq_dec s0 s); try congruence.
+        destruct (ground_maps.Raw.find (elt:= list (list ground_types)) s0 this) eqn:F.
+        unfold gt_set_type. rewrite F.
+        eapply Bool.andb_true_iff in H1. destruct H1.
+        enough (List_Ground_Type_as_OT.eqb g1 l = true -> g1 = l).
+        eapply H3 in H1. subst. reflexivity.
+        admit.
+        simpl in H1. congruence.
+        admit.
+      * subst.
+        enough ((ground_maps.Raw.check
+            (fun e' e : list (list ground_types) =>
+             List_Ground_Type_as_OT.eqb e e') s g0 
+            ((s0, g1) :: g) && true)%bool = true).
+        eapply Bool.andb_true_iff in H1.
+        destruct H1.
+        unfold ground_maps.Raw.check in H1.
+        simpl in H1. destruct (String_as_OT.eq_dec s s0); try congruence.
+        destruct (ground_maps.Raw.find (elt:= list (list ground_types)) s g) eqn:F.
+        unfold gt_set_type. rewrite F. unfold List_Ground_Type_as_OT.eqb in H1.
+        destruct (List_Ground_Type_as_OT.Inner.eq_dec l g0). subst. reflexivity.
+        congruence.
+        congruence.
+        admit.
+      * f_equal.
+        invs NoDup. invs NoDup0.
+        enough (ground_maps.Equal ({| ground_maps.this := g;
+                                     ground_maps.NoDup := H4 |})
+                                  ({| ground_maps.this := this;
+                                     ground_maps.NoDup := H6 |})).
+        eapply ground_maps_equality in H1. invs H1. reflexivity.
+        unfold ground_maps.Equal.
+        intros.
+        enough (ground_maps.equal List_Ground_Type_as_OT.eqb
+                                  {| ground_maps.this := g; ground_maps.NoDup := H4 |}
+                                  {| ground_maps.this := this; ground_maps.NoDup := H6 |} = true).
+        eapply IHg in H1.
+        eapply H1.
+        unfold ground_maps.equal. unfold ground_maps.Raw.equal.
+        unfold ground_maps.Raw.submap.
+        eapply Bool.andb_true_iff.
+        split.
+        -- admit.
+           
+           
+        
+      
+      
+      
+    
+                               
+Admitted.
+
+Lemma ground_maps_NEqual_implies_nequal :
+  forall (g g': gm_type),
+    ~ ground_maps.Equal (elt:=gt_set_type) g g' <->
+      ground_maps.equal List_Ground_Type_as_OT.eqb g g' = false.
+Proof.
+Admitted.
+
+
+Lemma program_semantics_adequacy' :
+  forall (rulez: list (string * rel * monotone_ops)) (g g': gm_type),
+    Forall
+      (fun elmt : OrdersEx.String_as_OT.t * rel * monotone_ops =>
+         let (y, _) := elmt in let (n, r) := y in n = name r) rulez ->
+
+    program_semantics g rulez g' ->
+    exists fuel,
+      program_semantics_eval_helper g rulez fuel = Some g'.
+Proof.
+  intros rulez g g' F P.
+  dependent induction P; intros.
+  - exists 1. simpl.
+    eapply rule_semantics_adequacy in H; try eassumption. rewrite <- H.
+    eapply ground_maps_Equal_implies_equal in H0. rewrite H0. reflexivity.
+  - specialize (IHP F). destruct IHP as (fuel & IHP).
+    exists (S fuel).
+    simpl.
+    eapply rule_semantics_adequacy in H; eauto.
+    rewrite <- H.
+    eapply ground_maps_NEqual_implies_nequal in H0. rewrite H0.
+    eassumption.
+Qed.
+
+Lemma program_semantics_adequacy :
+  forall (fuel: nat) (rulez: list (string * rel * monotone_ops)) (g g': gm_type),
+    Forall
+      (fun elmt : OrdersEx.String_as_OT.t * rel * monotone_ops =>
+         let (y, _) := elmt in let (n, r) := y in n = name r) rulez ->
+
+    program_semantics_eval_helper g rulez fuel = Some g' ->
+    program_semantics g rulez g'.
+Proof.
+  induction fuel; intros rulez g g' F P.
+  - simpl in P. inversion P.
+  - simpl in P.
+    symmetry in P. destruct_hyp_match.
+    destruct (ground_maps.equal List_Ground_Type_as_OT.eqb g g0) eqn:E.
+    + eapply ground_maps_Equal_implies_equal in E.
+      invc P.
+      eapply ground_maps_equality in E. subst.
+      econstructor. eapply rule_semantics_adequacy; eauto.
+      split; intros; eauto.
+    + eapply ground_maps_NEqual_implies_nequal in E.
+      eapply program_step_continue.
+      * eapply rule_semantics_adequacy; eauto.
+      * eassumption.
+      * eapply IHfuel; eauto.
+Qed.
+
+Lemma fold_left_construction :
+  forall v1 v1' init R,
+    fold_left
+      (fun (acc : set str_gt_list_ot.t) (elmt : list ground_types) =>
+         match variable_list_groundings_to_assoc_list R elmt with
+         | Some l => set_add str_gt_list_ot.eq_dec l acc
+         | None => acc
+         end) v1 init = v1' ->
+    v1' = init ++ (fold_left
+                     (fun (acc : set str_gt_list_ot.t) (elmt : list ground_types) =>
+                        match variable_list_groundings_to_assoc_list R elmt with
+                        | Some l => set_add str_gt_list_ot.eq_dec l acc
+                        | None => acc
+                        end) v1 nil).
+Proof.
+  induction v1; intros.
+  - simpl in H. subst. simpl. rewrite app_nil_r. reflexivity.
+  - simpl in H. eapply IHv1 in H. rewrite H.
+    symmetry.
+    match goal with
+    | [ |- _ = match ?x with
+              | Some _ => _
+              | None => init
+              end ++ _ ] =>
+        destruct (x) eqn:X
+    end.
+    + simpl. rewrite X.
+      match goal with
+      | [ |- init ++ ?a = _ ] =>
+          remember (a) as y
+      end.
+      symmetry in Heqy.
+      eapply IHv1 in Heqy. subst.
+      eapply list_set_equality.
+      simpl. intros.
+      split; intros.
+      * eapply in_app_or in H. destruct H.
+        -- eapply in_or_app. left. eapply set_add_iff. right. eassumption.
+        -- simpl in H. destruct H.
+           ++ subst. eapply in_or_app. left. eapply set_add_iff. left. reflexivity.
+           ++ eapply in_or_app. right. eassumption.
+      * eapply in_app_or in H. destruct H.
+        -- eapply set_add_elim in H. destruct H.
+           ++ subst. eapply in_or_app. right. simpl. left. reflexivity.
+           ++ eapply in_or_app. left. eauto.
+        -- eapply in_or_app. right. simpl. right. eassumption.
+    + simpl. rewrite X. reflexivity.
+Qed.
+
+Lemma assign_vars_to_tuples_monotone :
+  forall (R: rel) (v1 v2: list (list ground_types)) (v1' v2': tup_set),
+    list_set_subset v1 v2 ->
+    assign_vars_to_tuples R v1 = v1' ->
+    assign_vars_to_tuples R v2 = v2' ->
+    list_set_subset v1' v2'.
+Proof.
+  intros R. induction v1; intros.
+  - simpl in H0. invs H0. simpl. intros. invs H0.
+  - simpl in H.
+    assert (set_In a v2).
+    {
+      eapply H. left. reflexivity.
+    }
+    assert (list_set_subset v1 v2).
+    {
+      simpl. intros. eapply H. right. eassumption.
+    }
+    simpl in H0.
+    destruct (variable_list_groundings_to_assoc_list R a) eqn:A.
+    pose proof (fold_left_construction).
+    specialize (H4 _ _ _ _ H0). rewrite H4. rewrite <- H1. simpl. intros.
+    destruct H5.
+    + subst.
+      assert (v2 = a :: v2).
+      {
+        (* this normally wouldn't be possible but since we're treating these kinds of lists as sets, this is "fine" *)
+        eapply list_set_equality.
+        simpl. split; intros.
+        - destruct (List_Ground_Type_as_OTF.eq_dec a x0).
+          invs e. left. reflexivity.
+          right. eassumption.
+        - destruct H0; subst; eassumption.
+      }
+      rewrite H0. clear H0.
+      simpl. rewrite A.
+      match goal with
+      | [ |- set_In _ ?a] =>
+          remember (a) as A1
+      end.
+      symmetry in HeqA1.
+      eapply fold_left_construction in HeqA1.
+      subst.
+      eapply in_or_app.
+      left. simpl. left. reflexivity.
+    + unfold empty_set.
+      eapply IHv1. eapply H3. reflexivity. reflexivity.
+      eassumption.
+    + unfold empty_set in H0. rewrite <- H0.
+      simpl. intros.
+      rewrite <- H1. simpl. eapply IHv1. eapply H3. reflexivity. reflexivity.
+      eapply H4.
+Qed.
+
+Lemma select_relation_fold_app :
+  forall v init var val,
+    set_fold_left (select_relation_f var val) v init =
+      init ++ set_fold_left (select_relation_f var val) v nil.
+Proof.
+  induction v; intros.
+  - simpl. rewrite app_nil_r. reflexivity.
+  - Opaque select_relation_f.
+    simpl. rewrite IHv. symmetry. rewrite IHv. symmetry.
+    eapply list_set_equality.
+    simpl. split; intros; eapply in_app_or in H.
+    + destruct H.
+      * 
+        Transparent select_relation_f.
+        Opaque select_tuples.
+        simpl in H.
+        match goal with
+        | [ H: List.In x (match ?y with | Some _ => _ | None => init end) |- _ ] =>
+            destruct (y) eqn:Y
+        end.
+        -- simpl.
+           rewrite Y.
+           eapply in_or_app.
+           eapply set_add_elim in H. destruct H; subst.
+           ++ right. eapply in_or_app. left. left; reflexivity.
+           ++ left. eassumption.
+        -- eapply in_or_app. left. eassumption.
+      * eapply in_or_app. right. eapply in_or_app. right. eassumption.
+    + simpl. destruct (select_tuples var val a) eqn:Y.
+      * simpl in H. rewrite Y in H.
+        eapply in_or_app. destruct H.
+        -- left. eapply set_add_iff. right. eassumption.
+        -- eapply in_app_or in H. destruct H.
+           ++ left. eapply set_add_iff. left. simpl in H. destruct H; try congruence. contradiction.
+           ++ right. eassumption.
+      * eapply in_or_app. destruct H.
+        -- left. eassumption.
+        -- eapply in_app_or in H. simpl in H. rewrite Y in H. simpl in H.
+           destruct H; try contradiction.
+           right. eassumption.
+Qed.
+
+
+
+Lemma select_relation_monotone :
+  forall v v0 var val,
+    list_set_subset v v0 ->
+    list_set_subset (select_relation var val v) (select_relation var val v0).
+Proof.
+  induction v; intros.
+  - simpl. intros. invs H0.
+  - Opaque select_relation_f.
+    unfold select_relation. simpl. intros.
+    rewrite select_relation_fold_app in H0.
+    assert (v0 = a :: v0).
+    {
+      simpl in H. eapply list_set_equality.
+      simpl. split; intros.
+      - right. eassumption.
+      - destruct H1; subst.
+        + eapply H. left. reflexivity.
+        + eassumption.
+    }
+    rewrite H1.
+    simpl. rewrite select_relation_fold_app.
+    
+    eapply in_or_app.
+    eapply in_app_or in H0. destruct H0.
+    + left. Transparent select_relation_f. simpl in H0. simpl.
+      destruct (select_tuples var val a) eqn:Y. clear H1.
+      * eapply H0.
+      * invs H0.
+    + clear H1. right. eapply IHv.
+      * simpl. intros. eapply H. simpl. right. eassumption.
+      * eapply H0.
+Qed.
+
+Lemma proj_relation_fold_None' :
+  forall v init proj_vars,
+    set_fold_left
+      (fun (acc : option (set tup_type)) (elmt : tup_type) =>
+         match proj_tuples proj_vars elmt with
+         | Some tup => option_map (set_add str_gt_list_ot.eq_dec tup) acc
+         | None => None
+         end) v (Some init) = None <->
+      proj_relation proj_vars v = None.
+Proof.
+  induction v; split; intros.
+  - simpl in H. invs H.
+  - simpl in H. invs H.
+  - Opaque proj_tuples. simpl in H. destruct (proj_tuples proj_vars a) eqn:A.
+    + unfold tup_type in *. eapply IHv in H. simpl.
+      rewrite A. eapply IHv. eassumption.
+    + simpl. rewrite A. rewrite H. reflexivity.
+  - simpl in H. simpl. destruct (proj_tuples proj_vars a) eqn:A.
+    + eapply IHv in H. eapply IHv. eassumption.
+    + eassumption.
+Qed.
+
+Lemma proj_relation_fold_None :
+  forall v proj_vars,
+    set_fold_left
+      (fun (acc : option (set tup_type)) (elmt : tup_type) =>
+         match proj_tuples proj_vars elmt with
+         | Some tup => option_map (set_add str_gt_list_ot.eq_dec tup) acc
+         | None => None
+         end) v None = None.
+Proof.
+  induction v; intros.
+  - reflexivity.
+  - simpl. destruct (proj_tuples proj_vars a).
+    + rewrite IHv. reflexivity.
+    + rewrite IHv. reflexivity.
+Qed.
+
+
+Lemma proj_tuples_fold_app :
+  forall v v1 init proj_vars,
+    set_fold_left
+      (fun (acc : option (set tup_type)) (elmt : tup_type) =>
+         match proj_tuples proj_vars elmt with
+         | Some tup => option_map (set_add str_gt_list_ot.eq_dec tup) acc
+         | None => None
+         end) v (Some init) = Some v1 ->
+    Some v1 = option_map_map (@app (tup_type))
+                             (Some init)
+                             (proj_relation proj_vars v).
+Proof.
+  induction v; intros.
+  - simpl in H. invs H. simpl. unfold empty_set. rewrite app_nil_r. reflexivity.
+  - simpl in H. destruct (proj_tuples proj_vars a) eqn:A.
+    + eapply IHv in H.
+      simpl. rewrite A.
+      destruct_goal_match.
+      * eapply IHv in X. replace (Some (init ++ s)) with (option_map_map (app (A:= tup_type)) (Some init) (Some s)) by reflexivity.
+        rewrite H. rewrite X.
+        Opaque proj_relation.
+        simpl.
+        destruct (proj_relation proj_vars v) eqn:P.
+        -- f_equal. eapply list_set_equality.
+           simpl. split; intros.
+           ++ eapply in_app_or in H0. eapply in_or_app.
+              destruct H0.
+              ** eapply set_add_iff in H0. destruct H0; subst.
+                 --- right. left; eauto.
+                 --- left. eauto.
+              ** right. right; eauto.
+           ++ eapply in_app_or in H0. eapply in_or_app.
+              destruct H0.
+              ** left. eapply set_add_iff. right. eassumption.
+              ** simpl in H0. destruct H0; subst.
+                 --- left. eapply set_add_iff. left. eauto.
+                 --- right. eauto.
+        -- reflexivity.
+      * pose proof (proj_relation_fold_None').
+        eapply H0 in X. rewrite X in H. invs H.
+    + rewrite proj_relation_fold_None in H. invs H.
+Qed.
+
+
+Lemma proj_relation_monotone :
+  forall v v0 v1 v2 proj_vars,
+    list_set_subset v v0 ->
+    proj_relation proj_vars v = Some v1 ->
+    proj_relation proj_vars v0 = Some v2 ->
+    list_set_subset v1 v2.
+Proof.
+  induction v; intros.
+  - simpl in H0. invs H0. simpl. intros. invs H2.
+  - simpl in H0.
+    assert (v0 = a :: v0).
+    {
+      eapply list_set_equality.
+      simpl; split; intros.
+      - right. eassumption.
+      - destruct H2; subst.
+        + eapply H. left; reflexivity.
+        + eassumption.
+    }
+    rewrite H2 in H1. clear H2.
+    simpl. intros.
+    destruct (proj_tuples proj_vars a) eqn:A.
+    + Transparent proj_relation. simpl in H1.
+      rewrite A in H1.
+      simpl in H0. rewrite A in H0.
+      eapply proj_tuples_fold_app in H1. eapply proj_tuples_fold_app in H0.
+      assert (list_set_subset v v0).
+      {
+        simpl. intros.
+        eapply H. right. eassumption.
+      }
+      destruct (proj_relation proj_vars v) eqn:V; destruct (proj_relation proj_vars v0) eqn:V0.
+      * specialize (IHv v0 s s0).
+        specialize (IHv _ H3 V V0).
+        simpl in H0. simpl in H1. invs H0. invs H1. simpl in H2. destruct H2; subst.
+        -- left; reflexivity.
+        -- right; eauto.
+      * simpl in H1. congruence.
+      * simpl in H0. congruence.
+      * simpl in H0. congruence.
+    + simpl in H0. rewrite A in H0.
+      rewrite proj_relation_fold_None in H0.
+      invs H0.
+Qed.
+
+Lemma join_fold_app :
+  forall v init join_vars,
+    fold_left
+      (fun (acc : set tup_type) (elmt : tup_type * tup_type) =>
+         let (t1, t2) := elmt in
+         match join_tuples join_vars t1 t2 with
+         | Some tup => set_add str_gt_list_ot.eq_dec tup acc
+         | None => acc
+         end) v init =
+      init ++ fold_left
+           (fun (acc : set tup_type) (elmt : tup_type * tup_type) =>
+              let (t1, t2) := elmt in
+              match join_tuples join_vars t1 t2 with
+              | Some tup => set_add str_gt_list_ot.eq_dec tup acc
+              | None => acc
+              end) v nil .
+Proof.
+  induction  v; intros.
+  - simpl. rewrite app_nil_r. reflexivity.
+  - Opaque join_tuples. simpl. destruct a; destruct (join_tuples join_vars t t0) eqn:J.
+    + rewrite IHv. symmetry. rewrite IHv.
+      eapply list_set_equality.
+      split; intros.
+      * eapply in_app_or in H. eapply in_or_app.
+        destruct H.
+        -- left. eapply set_add_iff. right. eauto.
+        -- eapply in_app_or in H. destruct H.
+           ++ destruct H; subst; try contradiction.
+              left. eapply set_add_iff. left. eauto.
+           ++ right. eauto.
+      * eapply in_app_or in H. eapply in_or_app.
+        destruct H.
+        -- eapply set_add_iff in H. destruct H; subst.
+           ++ right. eapply in_or_app. left. left; eauto.
+           ++ left. eauto.
+        -- right. eapply in_or_app. right. eauto.
+    + eapply IHv.
+Qed.
+
+
+Lemma join_fold_monotone :
+  forall v v' v0 v0' join_vars,
+    list_set_subset v v0 ->
+    fold_left
+      (fun (acc : set tup_type) (elmt : tup_type * tup_type) =>
+         let (t1, t2) := elmt in
+         match join_tuples join_vars t1 t2 with
+         | Some tup => set_add str_gt_list_ot.eq_dec tup acc
+         | None => acc
+         end) v nil = v' ->
+    fold_left
+      (fun (acc : set tup_type) (elmt : tup_type * tup_type) =>
+         let (t1, t2) := elmt in
+         match join_tuples join_vars t1 t2 with
+         | Some tup => set_add str_gt_list_ot.eq_dec tup acc
+         | None => acc
+         end) v0 nil = v0' ->
+    list_set_subset v' v0'.
+Proof.
+  induction v; intros.
+  - simpl in H0. subst.
+    Opaque join_tuples.
+    simpl. intros. contradiction.
+  - simpl in H0. destruct a. destruct (join_tuples join_vars t t0) eqn:J.
+    + assert (v0 = (t, t0) :: v0).
+      {
+        eapply list_set_equality.
+        simpl; split; intros.
+        - right. eauto.
+        - destruct H2; subst.
+          + eapply H. left; reflexivity.
+          + eauto.
+      }
+      rewrite H2 in H1. clear H2.
+      simpl in H1.
+      rewrite J in H1.
+      rewrite join_fold_app in H1. rewrite join_fold_app in H0. rewrite <- H0. rewrite <- H1.
+      simpl. intros. destruct H2.
+      * left. eauto.
+      * right. eapply IHv.
+        simpl. intros. eapply H. right. eassumption.
+        reflexivity. reflexivity. eassumption.
+    + rewrite <- H0. rewrite <- H1. eapply IHv. simpl. intros. eapply H. right. eauto.
+      reflexivity. reflexivity.
+Qed.
+
+Print join_relations.
+
+Lemma set_prod_helper {A: Type}  {B: Type} :
+  forall (v3: set B) t t0 (a: A),
+    In (t, t0) (map (fun y => (a, y)) v3) <->
+    t = a /\ In t0 v3.
+Proof.
+  induction v3; split; intros.
+  - invs H.
+  - destruct H. invs H0.
+  - simpl in H. destruct H.
+    + invs H. split; intros.
+      * reflexivity.
+      * left. reflexivity.
+    + eapply IHv3 in H. destruct H. split; eauto.
+      right; eauto.
+  - destruct H. simpl in H0. subst.
+    destruct H0; subst.
+    + simpl. left. reflexivity.
+    + simpl. right. eapply IHv3. split; eauto.
+Qed.
+
+Lemma set_prod_in_iff {A B: Type} :
+  forall (v1: set A) (v2: set B) (a: A) (b: B),
+    In (a, b) (set_prod v1 v2) <->
+      In a v1 /\ In b v2.
+Proof.
+  induction v1; split; intros.
+  - invs H.
+  - destruct H. invs H.
+  - simpl in H. eapply in_app_iff in H. destruct H.
+    + eapply set_prod_helper in H. destruct H; subst.
+      split; eauto. left. eauto.
+    + eapply IHv1 in H. destruct H. split; eauto.
+      right. eauto.
+  - simpl in H. destruct H. simpl. eapply in_app_iff.
+    destruct H.
+    + subst. left. eapply set_prod_helper. split; eauto.
+    + right. eapply IHv1. split; eauto.
+Qed.
+
+Lemma set_prod_monotone :
+  forall (v0 v1 v3 v4: set tup_type),
+    list_set_subset v0 v1 ->
+    list_set_subset v3 v4 ->
+    list_set_subset (set_prod v0 v3) (set_prod v1 v4).
+Proof.
+  induction v0; intros.
+  - simpl. intros. contradiction.
+  - simpl. simpl in H.
+    assert (list_set_subset v0 v1).
+    {
+      simpl. intros. eapply H. right. eassumption.
+    }
+    specialize (IHv0 _ _ _ H1 H0).
+    intros. eapply in_app_iff in H2. destruct H2.
+    + destruct x. eapply set_prod_helper in H2.
+      destruct H2.
+      subst. eapply set_prod_in_iff.
+      split.
+      * eapply H. left. reflexivity.
+      * eapply H0. eassumption.
+    + destruct x. eapply set_prod_in_iff. eapply set_prod_in_iff in H2.
+      destruct H2. simpl in H0. simpl in H1.
+      split; eauto.
+      * eapply H1. eauto.
+      * eapply H0. eauto.
+Qed.
+
+Lemma join_relations_monotone :
+  forall v0 v1 v3 v4 join_vars,
+    list_set_subset v0 v1 ->
+    list_set_subset v3 v4 ->
+    list_set_subset (join_relations join_vars v0 v3)
+                    (join_relations join_vars v1 v4).
+Proof.
+  induction v0; intros.
+  - Opaque join_tuples. simpl.
+    intros. contradiction.
+  - assert (v1 = a :: v1).
+    { eapply list_set_equality.
+      simpl; split; intros.
+      - right. eassumption.
+      - destruct H1; subst.
+        + eapply H. left; reflexivity.
+        + eauto.
+    }
+    rewrite H1.
+    unfold join_relations.
+    eapply join_fold_monotone.
+    eapply set_prod_monotone.
+    rewrite H1 in H. eapply H. eapply H0. reflexivity. reflexivity.
+Qed.
+
+
+
+
+
+
+Lemma monotone_op_semantics_monotone :
+  forall (m: monotone_ops) (g1 g2: gm_type) (v1 v2: tup_set),
+    ground_map_Subset g1 g2 ->
+    monotone_op_semantics g1 m v1 ->
+    monotone_op_semantics g2 m v2 ->
+    list_set_subset v1 v2.
+Proof.
+  induction m; intros.
+  - inversion H0.
+  - invs H0.
+    invs H1.
+    simpl in H. destruct H.
+    specialize (H2 _ _ _ H4 H5). simpl.
+    intros. eapply assign_vars_to_tuples_monotone. simpl. eapply H2. reflexivity. reflexivity.
+    eapply H3.
+  - invs H0. invs H1.
+    specialize (IHm _ _ _ _ H H7 H8).
+    eapply select_relation_monotone. eassumption.
+  - invs H0. invs H1.
+    specialize (IHm1 _ _ _ _ H H4 H5).
+    specialize (IHm2 _ _ _ _ H H6 H8).
+    simpl. intros. eapply set_union_iff in H2. eapply set_union_iff.
+    destruct H2.
+    + left. eapply IHm1. eassumption.
+    + right. eapply IHm2. eauto.
+  - invs H0. invs H1.
+    specialize (IHm _ _ _ _ H H5 H6).
+    eapply proj_relation_monotone; eauto.
+  - invs H0. invs H1.
+    specialize (IHm1 _ _ _ _ H H6 H7).
+    specialize (IHm2 _ _ _ _ H H8 H10).
+    eapply join_relations_monotone; eauto.
+Qed.
+
+Print ground_maps.In.
+Print ground_maps.add.
+
+
+(* HERE *)
+        
+
+
+Lemma rule_semantics_monotone :
+  forall (rulez: list (string * rel * monotone_ops)) (g1 g2 g1' g2': gm_type),
+    ground_map_Subset g1 g2 ->
+    rule_semantics g1 rulez g1' ->
+    rule_semantics g2 rulez g2' ->
+    ground_map_Subset g1' g2'.
+Proof.
+  induction rulez; intros.
+  - invs H0. invs H1. eassumption.
+  - invs H0. invs H1.
+    clear H9.
+    pose proof (monotone_op_semantics_monotone).
+    specialize (H2 _ _ _ _ _ H H5 H10).
+    eapply IHrulez. shelve.
+    eapply H11.
+    eapply H17.
+    Unshelve.
+    Opaque set_union. simpl. split; intros.
+    + pose proof (ground_maps.add_1).
+      eapply ground_maps_add_iff.
+      eapply ground_maps_add_iff in H3.
+      destruct H3; try subst.
+      * left. reflexivity.
+      * right. eapply H. eassumption.
+    + unfold ground_map_Subset in H.
+      destruct H.
+      eapply ground_maps.find_2 in H3.
+      eapply ground_maps.find_2 in H4.
+
+      unfold ground_maps.MapsTo in *. simpl in H3, H4.
+      eapply ground_maps_raw_MapsTo_add_iff in H3, H4.
+      destruct H3, H4.
+      * destruct H3, H4.
+        subst.
+        eapply set_union_elim in H8. eapply set_union_iff.
+        destruct H8.
+        admit.
+        admit.
+      * destruct H4. destruct H3. congruence.
+      * destruct H3, H4. congruence.
+      * destruct H3, H4.
+        eapply H9.
+        eapply ground_maps.find_1. eauto. eapply ground_maps.find_1. eauto. eauto.
+      * eapply (ground_maps.NoDup g2).
+      * eapply (ground_maps.NoDup g1).
+Admitted.
+
+(* need equivalent of set_add_iff *)
+
+Lemma rule_semantics_increasing :
+  forall (rulez: list (string * rel * monotone_ops)) (g1 g2: gm_type),
+    rule_semantics g1 rulez g2 ->
+    ground_map_Subset g1 g2.
+Proof.
+  induction rulez; intros.
+  - invs H. simpl. split; intros; eauto.
+    rewrite H1 in H0. invs H0. eauto.
+  - invs H.
+    eapply IHrulez in H9.
+    simpl. simpl in H9.
+    split; intros.
+    + destruct H9.
+      eapply H1. unfold ground_maps.In in *. unfold ground_maps.Raw.PX.In in *. destruct H0.
+      destruct (String_as_OT.eq_dec x (name R)).
+      * subst. exists (set_union List_Ground_Type_as_OTF.eq_dec new_tuples
+                            old_tuples).
+        simpl. eapply ground_maps_raw_MapsTo_add_iff.
+        eapply (ground_maps.NoDup g1).
+        left. eauto.
+      * exists x0. eapply ground_maps_raw_MapsTo_add_iff.
+        eapply (ground_maps.NoDup g1).
+        right. split; eauto.
+    + destruct (String_as_OT.eq_dec x (name R)).
+      * subst.
+        destruct H9. eapply H7.
+        eapply ground_maps.find_1.
+        eapply ground_maps.find_2 in H1, H0.
+        unfold ground_maps.MapsTo. eapply ground_maps_raw_MapsTo_add_iff.
+        eapply (ground_maps.NoDup g1).
+        left. split; reflexivity.
+        eauto.
+        rewrite <- H5 in H0. invs H0. eapply set_union_iff. right. eauto.
+      * destruct H9. eapply H7.
+        eapply ground_maps.find_1. unfold ground_maps.MapsTo. simpl. eapply ground_maps_raw_MapsTo_add_iff.
+        eapply (ground_maps.NoDup g1).
+        right. split; eauto.
+        eapply ground_maps.find_2. eauto. eauto.
+        eauto.
+Qed.
+
+Lemma ground_map_Subset_transitive :
+  forall g1 g2 g3,
+    ground_map_Subset g1 g2 ->
+    ground_map_Subset g2 g3 ->
+    ground_map_Subset g1 g3.
+Proof.
+  intros.
+  destruct H as (G1k & G1v). destruct H0 as (G2k & G2v).
+  simpl. split; intros.
+  - eapply G2k. eapply G1k.
+    eauto.
+  - eapply ground_maps.find_2 in H, H0.
+    unfold ground_maps.In in *. unfold ground_maps.MapsTo in *.
+    unfold ground_maps.Raw.PX.In in *.
+    assert (exists e, ground_maps.Raw.PX.MapsTo x e (ground_maps.this g1)).
+    exists l1. eauto.
+    eapply G1k in H2. destruct H2.
+    pose proof (ground_maps_MapsTo_det).
+    eapply G2v. eapply ground_maps.find_1. eauto. eapply ground_maps.find_1. eauto.
+    eapply G1v.
+    eapply ground_maps.find_1. eauto. eapply ground_maps.find_1. eauto. eauto.
+Qed.
+
+Lemma program_semantics_increasing :
+  forall (rulez: list (string * rel * monotone_ops)) (g1 g2: gm_type),
+    program_semantics g1 rulez g2 ->
+    ground_map_Subset g1 g2.
+Proof.
+  intros. induction H; intros.
+  - simpl. split; intros; eauto.
+    rewrite H1 in H2. invs H2. eauto.
+  - eapply ground_map_Subset_transitive.
+    eapply rule_semantics_increasing; eauto.
+    eauto.
+Qed.
+
+
+Lemma ground_maps_eq_refl :
+  forall (g: gm_type),
+    ground_maps.Equal g g.
+Proof.
+  intros.
+  unfold ground_maps.Equal.
+  intros. reflexivity.
+Qed.
+
+Lemma monotone_cannot_be_empty :
+  forall (m: monotone_ops) v,
+    monotone_op_semantics
+      (ground_maps.empty _) m v ->
+    False.
+Proof.
+  induction m; intros.
+  - invs H.
+  - invs H. unfold ground_maps.find in H2. simpl in H2. invs H2.
+  - invs H. eapply IHm in H5. contradiction.
+  - invs H. eapply IHm1 in H2. contradiction.
+  - invs H. eapply IHm in H3. contradiction.
+  - invs H. eauto.
+Qed.
+
+Lemma rule_semantics_cannot_be_empty :
+  forall (rulez: list (string * rel * monotone_ops)) (r: string * rel * monotone_ops) (g: gm_type),
+    rule_semantics
+      (ground_maps.empty _) (r :: rulez)
+      g ->
+    False.
+Proof.
+  induction rulez; intros.
+  - invs H. unfold ground_maps.find in H5. unfold ground_maps.Raw.find in H5. simpl in H5. invs H5.
+  - invs H.
+    invs H. eapply monotone_cannot_be_empty in H8. contradiction.
+Qed.
+
+Lemma program_semantics_monotone :
+  forall (rulez: list (string * rel * monotone_ops)) (g1 g2 g1' g2': gm_type),
+    program_semantics g1 rulez g1' ->
+    ground_map_Subset g1 g2 ->
+    program_semantics g2 rulez g2' ->
+    ground_map_Subset g1' g2'.
+Proof.
+  intros rulez g1 g2 g1' g2'.
+  intros P. revert g2 g2'. induction P; intros.
+  - eapply program_semantics_increasing in H2. eapply ground_map_Subset_transitive; eauto.
+  - invs H2.
+    + eapply ground_maps_equality in H4. subst.
+      invs P.
+      * eapply ground_maps_equality in H5. subst.
+        pose proof (rule_semantics_monotone).
+        specialize (H5 _ _ _ _ _ H1 H H3).
+        eauto.
+      * invs H6. eapply ground_maps_equality in H8. subst.
+        eapply rule_semantics_increasing in H4.
+        invs H3.
+        -- invs H. invs P. invs H8. eassumption.
+           invs H8. eapply IHP. eapply H1. eassumption.
+        -- pose proof (rule_semantics_monotone).
+           specialize (H8 _ _ _ _ _ H1 H H3).
+           specialize (IHP _ g'0 H8). eapply IHP in H2. eassumption.
+        -- pose proof (rule_semantics_monotone _ _ _ _ _ H1 H H3).
+           specialize (IHP _ g'0 H10 H2). eassumption.
+    + pose proof (rule_semantics_monotone _ _ _ _ _ H1 H H3).
+      specialize (IHP _ g2' H6 H5). eassumption.
+Qed.
+ 
