RuleSemanticsTheorems.v
@@ -1,0 +1,73 @@
+From Coq Require Import  List String Arith Psatz DecidableTypeEx OrdersEx Program.Equality FMapList FMapWeakList MSetWeakList Lists.ListSet.
+
+From VeriFGH Require Import DatalogSemantics.
+From VeriFGH Require Import OrdersFunctor DatalogProps StringOrders RelOrdered OrderedGroundTypes MoreOrders RelDecidable.
+
+Require Export MonotoneOpSemanticsTheorems.
+
+Import RelSemantics.
+
+
+Lemma rule_semantics_det :
+  forall (rules: list (string * rel * monotone_ops)) (g g1 g2: gm_type),
+    rule_semantics g rules g1 ->
+    rule_semantics g rules g2 ->
+    g1 = g2.
+Proof.
+  induction rules; intros.
+  - inversion H. inversion H0. subst. reflexivity.
+  - inversion H. subst. inversion H0. subst.
+    eapply IHrules. eassumption.
+    epose proof (monotone_op_semantics_det _ _ _ _ H4 H9).
+    subst.
+    rewrite <- H5 in H12. inversion H12. subst.
+    rewrite <- H6 in H14. inversion H14. subst. eassumption.
+Qed.
+
+Lemma rule_semantics_adequacy :
+  forall (rules: list (string * rel * monotone_ops)) (g g': gm_type),
+    Forall (fun elmt =>
+              match elmt with
+              | (n, r, m) => n = name r
+              end) rules ->
+    Some g' = rule_semantics_eval' g rules <->
+      rule_semantics g rules g'.
+Proof.
+  induction rules; intros; split; intros.
+  - inversion H0. econstructor.
+  - inversion H0. subst. reflexivity.
+  - simpl in H0. destruct a.  destruct p. destruct (string_dec (name r) s).
+    + destruct_hyp_match. destruct_hyp_match.
+      destruct_hyp_match.
+      econstructor. eassumption.
+      eapply monotone_op_semantics_adequacy. symmetry in X. eassumption.
+      symmetry in X0. eassumption.
+      
+      3: eapply IHrules in H3; inversion H; try eassumption.
+      2: reflexivity.
+      symmetry in X1. eassumption.
+    + inversion H. congruence.
+  - inversion H0. subst. inversion H. subst.
+    simpl. destruct (string_dec (name R) (name R)); try congruence.
+    clear e.
+    destruct_goal_match.
+    + destruct_goal_match.
+      * destruct_goal_match.
+        -- eapply IHrules in H10.
+           eapply monotone_op_semantics_adequacy in H4.
+           rewrite <- H4 in X. inversion X. subst.
+           clear X. rewrite X0 in H5. inversion H5. subst.
+           inversion H6. subst. eassumption.
+           eassumption.
+        -- inversion H6.
+      * eapply monotone_op_semantics_adequacy in H4. rewrite X in H4. inversion H4. subst. rewrite X0 in H5. congruence.
+    + eapply monotone_op_semantics_adequacy in H4. rewrite X in H4. congruence.
+Qed.
+
+(* States of reaching fixpoint:
+     have fuel -> run another iter -> maps are the same -> end
+                                   -> maps are not the same -> continue
+     don't have fuel -> fail
+
+
+ *)
